# baseURI: https://linkeddata.cultureelerfgoed.nl/def/ztco
# prefix: ztco

@prefix ceo: <https://linkeddata.cultureelerfgoed.nl/def/ceo#> .
@prefix dc: <http://purl.org/dc/elements/1.1/> .
@prefix dcam: <http://purl.org/dc/dcam/> .
@prefix dcterms: <http://purl.org/dc/terms/> .
@prefix foaf: <http://xmlns.com/foaf/0.1/> .
@prefix owl: <http://www.w3.org/2002/07/owl#> .
@prefix rdf: <http://www.w3.org/1999/02/22-rdf-syntax-ns#> .
@prefix rdfs: <http://www.w3.org/2000/01/rdf-schema#> .
@prefix skos: <http://www.w3.org/2004/02/skos/core#> .
@prefix xsd: <http://www.w3.org/2001/XMLSchema#> .
@prefix zo: <https://linkeddata.cultureelerfgoed.nl/def/zo#> .
@prefix ztco: <https://linkeddata.cultureelerfgoed.nl/def/ztco#> .

dc:
  dcterms:modified "2010-10-11" ;
  dcterms:publisher <http://purl.org/dc/aboutdcmi#DCMI> ;
  dcterms:title "Dublin Core Metadata Element Set, Version 1.1"@en-US ;
  rdfs:comment "This version has been modified for use in TopBraid: it defines the dc namespace prefix and imports SKOS and DCTerms." ;
.
dc:contributor
  a rdf:Property ;
  dcterms:description "Examples of a Contributor include a person, an organization, or a service. Typically, the name of a Contributor should be used to indicate the entity."@en-US ;
  dcterms:hasVersion <http://dublincore.org/usage/terms/history/#contributor-006> ;
  dcterms:issued "1999-07-02" ;
  dcterms:modified "2008-01-14" ;
  rdfs:comment "An entity responsible for making contributions to the resource."@en-US ;
  rdfs:isDefinedBy dc: ;
  rdfs:label "Contributor"@en-US ;
  skos:note "A second property with the same name as this property has been declared in the dcterms: namespace (http://purl.org/dc/terms/).  See the Introduction to the document \"DCMI Metadata Terms\" (http://dublincore.org/documents/dcmi-terms/) for an explanation."@en-US ;
.
dc:coverage
  a rdf:Property ;
  dcterms:description "Spatial topic and spatial applicability may be a named place or a location specified by its geographic coordinates. Temporal topic may be a named period, date, or date range. A jurisdiction may be a named administrative entity or a geographic place to which the resource applies. Recommended best practice is to use a controlled vocabulary such as the Thesaurus of Geographic Names [TGN]. Where appropriate, named places or time periods can be used in preference to numeric identifiers such as sets of coordinates or date ranges."@en-US ;
  dcterms:hasVersion <http://dublincore.org/usage/terms/history/#coverage-006> ;
  dcterms:issued "1999-07-02" ;
  dcterms:modified "2008-01-14" ;
  rdfs:comment "The spatial or temporal topic of the resource, the spatial applicability of the resource, or the jurisdiction under which the resource is relevant."@en-US ;
  rdfs:isDefinedBy dc: ;
  rdfs:label "Coverage"@en-US ;
  skos:note "A second property with the same name as this property has been declared in the dcterms: namespace (http://purl.org/dc/terms/).  See the Introduction to the document \"DCMI Metadata Terms\" (http://dublincore.org/documents/dcmi-terms/) for an explanation."@en-US ;
.
dc:creator
  a rdf:Property ;
  dcterms:description "Examples of a Creator include a person, an organization, or a service. Typically, the name of a Creator should be used to indicate the entity."@en-US ;
  dcterms:hasVersion <http://dublincore.org/usage/terms/history/#creator-006> ;
  dcterms:issued "1999-07-02" ;
  dcterms:modified "2008-01-14" ;
  rdfs:comment "An entity primarily responsible for making the resource."@en-US ;
  rdfs:isDefinedBy dc: ;
  rdfs:label "Creator"@en-US ;
  skos:note "A second property with the same name as this property has been declared in the dcterms: namespace (http://purl.org/dc/terms/).  See the Introduction to the document \"DCMI Metadata Terms\" (http://dublincore.org/documents/dcmi-terms/) for an explanation."@en-US ;
.
dc:date
  a rdf:Property ;
  dcterms:description "Date may be used to express temporal information at any level of granularity.  Recommended best practice is to use an encoding scheme, such as the W3CDTF profile of ISO 8601 [W3CDTF]."@en-US ;
  dcterms:hasVersion <http://dublincore.org/usage/terms/history/#date-006> ;
  dcterms:issued "1999-07-02" ;
  dcterms:modified "2008-01-14" ;
  rdfs:comment "A point or period of time associated with an event in the lifecycle of the resource."@en-US ;
  rdfs:isDefinedBy dc: ;
  rdfs:label "Date"@en-US ;
  skos:note "A second property with the same name as this property has been declared in the dcterms: namespace (http://purl.org/dc/terms/).  See the Introduction to the document \"DCMI Metadata Terms\" (http://dublincore.org/documents/dcmi-terms/) for an explanation."@en-US ;
.
dc:description
  a rdf:Property ;
  dcterms:description "Description may include but is not limited to: an abstract, a table of contents, a graphical representation, or a free-text account of the resource."@en-US ;
  dcterms:hasVersion <http://dublincore.org/usage/terms/history/#description-006> ;
  dcterms:issued "1999-07-02" ;
  dcterms:modified "2008-01-14" ;
  rdfs:comment "An account of the resource."@en-US ;
  rdfs:isDefinedBy dc: ;
  rdfs:label "Description"@en-US ;
  skos:note "A second property with the same name as this property has been declared in the dcterms: namespace (http://purl.org/dc/terms/).  See the Introduction to the document \"DCMI Metadata Terms\" (http://dublincore.org/documents/dcmi-terms/) for an explanation."@en-US ;
.
dc:format
  a rdf:Property ;
  dcterms:description "Examples of dimensions include size and duration. Recommended best practice is to use a controlled vocabulary such as the list of Internet Media Types [MIME]."@en-US ;
  dcterms:hasVersion <http://dublincore.org/usage/terms/history/#format-007> ;
  dcterms:issued "1999-07-02" ;
  dcterms:modified "2008-01-14" ;
  rdfs:comment "The file format, physical medium, or dimensions of the resource."@en-US ;
  rdfs:isDefinedBy dc: ;
  rdfs:label "Format"@en-US ;
  skos:note "A second property with the same name as this property has been declared in the dcterms: namespace (http://purl.org/dc/terms/).  See the Introduction to the document \"DCMI Metadata Terms\" (http://dublincore.org/documents/dcmi-terms/) for an explanation."@en-US ;
.
dc:identifier
  a rdf:Property ;
  dcterms:description "Recommended best practice is to identify the resource by means of a string conforming to a formal identification system. "@en-US ;
  dcterms:hasVersion <http://dublincore.org/usage/terms/history/#identifier-006> ;
  dcterms:issued "1999-07-02" ;
  dcterms:modified "2008-01-14" ;
  rdfs:comment "An unambiguous reference to the resource within a given context."@en-US ;
  rdfs:isDefinedBy dc: ;
  rdfs:label "Identifier"@en-US ;
  skos:note "A second property with the same name as this property has been declared in the dcterms: namespace (http://purl.org/dc/terms/).  See the Introduction to the document \"DCMI Metadata Terms\" (http://dublincore.org/documents/dcmi-terms/) for an explanation."@en-US ;
.
dc:language
  a rdf:Property ;
  dcterms:description "Recommended best practice is to use a controlled vocabulary such as RFC 4646 [RFC4646]."@en-US ;
  dcterms:hasVersion <http://dublincore.org/usage/terms/history/#language-007> ;
  dcterms:issued "1999-07-02" ;
  dcterms:modified "2008-01-14" ;
  rdfs:comment "A language of the resource."@en-US ;
  rdfs:isDefinedBy dc: ;
  rdfs:label "Language"@en-US ;
  rdfs:seeAlso <http://www.ietf.org/rfc/rfc4646.txt> ;
  skos:note "A second property with the same name as this property has been declared in the dcterms: namespace (http://purl.org/dc/terms/).  See the Introduction to the document \"DCMI Metadata Terms\" (http://dublincore.org/documents/dcmi-terms/) for an explanation."@en-US ;
.
dc:publisher
  a rdf:Property ;
  dcterms:description "Examples of a Publisher include a person, an organization, or a service. Typically, the name of a Publisher should be used to indicate the entity."@en-US ;
  dcterms:hasVersion <http://dublincore.org/usage/terms/history/#publisher-006> ;
  dcterms:issued "1999-07-02" ;
  dcterms:modified "2008-01-14" ;
  rdfs:comment "An entity responsible for making the resource available."@en-US ;
  rdfs:isDefinedBy dc: ;
  rdfs:label "Publisher"@en-US ;
  skos:note "A second property with the same name as this property has been declared in the dcterms: namespace (http://purl.org/dc/terms/).  See the Introduction to the document \"DCMI Metadata Terms\" (http://dublincore.org/documents/dcmi-terms/) for an explanation."@en-US ;
.
dc:relation
  a rdf:Property ;
  dcterms:description "Recommended best practice is to identify the related resource by means of a string conforming to a formal identification system. "@en-US ;
  dcterms:hasVersion <http://dublincore.org/usage/terms/history/#relation-006> ;
  dcterms:issued "1999-07-02" ;
  dcterms:modified "2008-01-14" ;
  rdfs:comment "A related resource."@en-US ;
  rdfs:isDefinedBy dc: ;
  rdfs:label "Relation"@en-US ;
  skos:note "A second property with the same name as this property has been declared in the dcterms: namespace (http://purl.org/dc/terms/).  See the Introduction to the document \"DCMI Metadata Terms\" (http://dublincore.org/documents/dcmi-terms/) for an explanation."@en-US ;
.
dc:rights
  a rdf:Property ;
  dcterms:description "Typically, rights information includes a statement about various property rights associated with the resource, including intellectual property rights."@en-US ;
  dcterms:hasVersion <http://dublincore.org/usage/terms/history/#rights-006> ;
  dcterms:issued "1999-07-02" ;
  dcterms:modified "2008-01-14" ;
  rdfs:comment "Information about rights held in and over the resource."@en-US ;
  rdfs:isDefinedBy dc: ;
  rdfs:label "Rights"@en-US ;
  skos:note "A second property with the same name as this property has been declared in the dcterms: namespace (http://purl.org/dc/terms/).  See the Introduction to the document \"DCMI Metadata Terms\" (http://dublincore.org/documents/dcmi-terms/) for an explanation."@en-US ;
.
dc:source
  a rdf:Property ;
  dcterms:description "The described resource may be derived from the related resource in whole or in part. Recommended best practice is to identify the related resource by means of a string conforming to a formal identification system."@en-US ;
  dcterms:hasVersion <http://dublincore.org/usage/terms/history/#source-006> ;
  dcterms:issued "1999-07-02" ;
  dcterms:modified "2008-01-14" ;
  rdfs:comment "A related resource from which the described resource is derived."@en-US ;
  rdfs:isDefinedBy dc: ;
  rdfs:label "Source"@en-US ;
  skos:note "A second property with the same name as this property has been declared in the dcterms: namespace (http://purl.org/dc/terms/).  See the Introduction to the document \"DCMI Metadata Terms\" (http://dublincore.org/documents/dcmi-terms/) for an explanation."@en-US ;
.
dc:subject
  a rdf:Property ;
  dcterms:description "Typically, the subject will be represented using keywords, key phrases, or classification codes. Recommended best practice is to use a controlled vocabulary. To describe the spatial or temporal topic of the resource, use the Coverage element."@en-US ;
  dcterms:hasVersion <http://dublincore.org/usage/terms/history/#subject-006> ;
  dcterms:issued "1999-07-02" ;
  dcterms:modified "2008-01-14" ;
  rdfs:comment "The topic of the resource."@en-US ;
  rdfs:isDefinedBy dc: ;
  rdfs:label "Subject"@en-US ;
  skos:note "A second property with the same name as this property has been declared in the dcterms: namespace (http://purl.org/dc/terms/).  See the Introduction to the document \"DCMI Metadata Terms\" (http://dublincore.org/documents/dcmi-terms/) for an explanation."@en-US ;
.
dc:title
  a rdf:Property ;
  dcterms:hasVersion <http://dublincore.org/usage/terms/history/#title-006> ;
  dcterms:issued "1999-07-02" ;
  dcterms:modified "2008-01-14" ;
  rdfs:comment "A name given to the resource."@en-US ;
  rdfs:isDefinedBy dc: ;
  rdfs:label "Title"@en-US ;
  skos:note "A second property with the same name as this property has been declared in the dcterms: namespace (http://purl.org/dc/terms/).  See the Introduction to the document \"DCMI Metadata Terms\" (http://dublincore.org/documents/dcmi-terms/) for an explanation."@en-US ;
.
dc:type
  a rdf:Property ;
  dcterms:description "Recommended best practice is to use a controlled vocabulary such as the DCMI Type Vocabulary [DCMITYPE]. To describe the file format, physical medium, or dimensions of the resource, use the Format element."@en-US ;
  dcterms:hasVersion <http://dublincore.org/usage/terms/history/#type-006> ;
  dcterms:issued "1999-07-02" ;
  dcterms:modified "2008-01-14" ;
  rdfs:comment "The nature or genre of the resource."@en-US ;
  rdfs:isDefinedBy dc: ;
  rdfs:label "Type"@en-US ;
  skos:note "A second property with the same name as this property has been declared in the dcterms: namespace (http://purl.org/dc/terms/).  See the Introduction to the document \"DCMI Metadata Terms\" (http://dublincore.org/documents/dcmi-terms/) for an explanation."@en-US ;
.
dcterms:
  dcterms:modified "2010-10-11" ;
  dcterms:publisher <http://purl.org/dc/aboutdcmi#DCMI> ;
  dcterms:title "DCMI Metadata Terms in the /terms/ namespace"@en-US ;
.
dcterms:Agent
  a dcterms:AgentClass ;
  a rdfs:Class ;
  dcterms:description "Examples of Agent include person, organization, and software agent."@en-US ;
  dcterms:hasVersion <http://dublincore.org/usage/terms/history/#Agent-001> ;
  dcterms:issued "2008-01-14" ;
  rdfs:comment "A resource that acts or has the power to act."@en-US ;
  rdfs:isDefinedBy dcterms: ;
  rdfs:label "Agent"@en-US ;
.
dcterms:AgentClass
  a rdfs:Class ;
  dcterms:description "Examples of Agent Class include groups seen as classes, such as students, women, charities, lecturers."@en-US ;
  dcterms:hasVersion <http://dublincore.org/usage/terms/history/#AgentClass-001> ;
  dcterms:issued "2008-01-14" ;
  rdfs:comment "A group of agents."@en-US ;
  rdfs:isDefinedBy dcterms: ;
  rdfs:label "Agent Class"@en-US ;
  rdfs:subClassOf dcterms:AgentClass ;
.
dcterms:BibliographicResource
  a rdfs:Class ;
  dcterms:hasVersion <http://dublincore.org/usage/terms/history/#BibliographicResource-001> ;
  dcterms:issued "2008-01-14" ;
  rdfs:comment "A book, article, or other documentary resource."@en-US ;
  rdfs:isDefinedBy dcterms: ;
  rdfs:label "Bibliographic Resource"@en-US ;
.
dcterms:Box
  a rdfs:Datatype ;
  dcterms:hasVersion <http://dublincore.org/usage/terms/history/#Box-003> ;
  dcterms:issued "2000-07-11" ;
  dcterms:modified "2008-01-14" ;
  rdfs:comment "The set of regions in space defined by their geographic coordinates according to the DCMI Box Encoding Scheme."@en-US ;
  rdfs:isDefinedBy dcterms: ;
  rdfs:label "DCMI Box"@en-US ;
  rdfs:seeAlso <http://dublincore.org/documents/dcmi-box/> ;
.
dcterms:DCMIType
  a dcam:VocabularyEncodingScheme ;
  dcterms:hasVersion <http://dublincore.org/usage/terms/history/#DCMIType-003> ;
  dcterms:issued "2000-07-11" ;
  dcterms:modified "2010-10-11" ;
  rdfs:comment "The set of classes specified by the DCMI Type Vocabulary, used to categorize the nature or genre of the resource."@en-US ;
  rdfs:isDefinedBy dcterms: ;
  rdfs:label "DCMI Type Vocabulary"@en-US ;
  rdfs:seeAlso <http://dublincore.org/documents/dcmi-type-vocabulary/> ;
  rdfs:seeAlso <http://purl.org/dc/dcmitype/> ;
.
dcterms:DDC
  a dcam:VocabularyEncodingScheme ;
  dcterms:hasVersion <http://dublincore.org/usage/terms/history/#DDC-003> ;
  dcterms:issued "2000-07-11" ;
  dcterms:modified "2008-01-14" ;
  rdfs:comment "The set of conceptual resources specified by the Dewey Decimal Classification."@en-US ;
  rdfs:isDefinedBy dcterms: ;
  rdfs:label "DDC"@en-US ;
  rdfs:seeAlso <http://www.oclc.org/dewey/> ;
.
dcterms:FileFormat
  a rdfs:Class ;
  dcterms:description "Examples include the formats defined by the list of Internet Media Types."@en-US ;
  dcterms:hasVersion <http://dublincore.org/usage/terms/history/#FileFormat-001> ;
  dcterms:issued "2008-01-14" ;
  rdfs:comment "A digital resource format."@en-US ;
  rdfs:isDefinedBy dcterms: ;
  rdfs:label "File Format"@en-US ;
  rdfs:subClassOf dcterms:MediaType ;
.
dcterms:Frequency
  a rdfs:Class ;
  dcterms:hasVersion <http://dublincore.org/usage/terms/history/#Frequency-001> ;
  dcterms:issued "2008-01-14" ;
  rdfs:comment "A rate at which something recurs."@en-US ;
  rdfs:isDefinedBy dcterms: ;
  rdfs:label "Frequency"@en-US ;
.
dcterms:IMT
  a dcam:VocabularyEncodingScheme ;
  dcterms:hasVersion <http://dublincore.org/usage/terms/history/#IMT-004> ;
  dcterms:issued "2000-07-11" ;
  dcterms:modified "2008-01-14" ;
  rdfs:comment "The set of media types specified by the Internet Assigned Numbers Authority."@en-US ;
  rdfs:isDefinedBy dcterms: ;
  rdfs:label "IMT"@en-US ;
  rdfs:seeAlso <http://www.iana.org/assignments/media-types/> ;
.
dcterms:ISO3166
  a rdfs:Datatype ;
  dcterms:hasVersion <http://dublincore.org/usage/terms/history/#ISO3166-004> ;
  dcterms:issued "2000-07-11" ;
  dcterms:modified "2008-01-14" ;
  rdfs:comment "The set of codes listed in ISO 3166-1 for the representation of names of countries."@en-US ;
  rdfs:isDefinedBy dcterms: ;
  rdfs:label "ISO 3166"@en-US ;
  rdfs:seeAlso <http://www.iso.org/iso/en/prods-services/iso3166ma/02iso-3166-code-lists/list-en1.html> ;
.
dcterms:ISO639-2
  a rdfs:Datatype ;
  dcterms:hasVersion <http://dublincore.org/usage/terms/history/#ISO639-2-003> ;
  dcterms:issued "2000-07-11" ;
  dcterms:modified "2008-01-14" ;
  rdfs:comment "The three-letter alphabetic codes listed in ISO639-2 for the representation of names of languages."@en-US ;
  rdfs:isDefinedBy dcterms: ;
  rdfs:label "ISO 639-2"@en-US ;
  rdfs:seeAlso <http://lcweb.loc.gov/standards/iso639-2/langhome.html> ;
.
dcterms:ISO639-3
  a rdfs:Datatype ;
  dcterms:hasVersion <http://dublincore.org/usage/terms/history/#ISO639-3-001> ;
  dcterms:issued "2008-01-14" ;
  rdfs:comment "The set of three-letter codes listed in ISO 639-3 for the representation of names of languages."@en-US ;
  rdfs:isDefinedBy dcterms: ;
  rdfs:label "ISO 639-3"@en-US ;
  rdfs:seeAlso <http://www.sil.org/iso639-3/> ;
.
dcterms:Jurisdiction
  a rdfs:Class ;
  dcterms:hasVersion <http://dublincore.org/usage/terms/history/#Jurisdiction-001> ;
  dcterms:issued "2008-01-14" ;
  rdfs:comment "The extent or range of judicial, law enforcement, or other authority."@en-US ;
  rdfs:isDefinedBy dcterms: ;
  rdfs:label "Jurisdiction"@en-US ;
  rdfs:subClassOf dcterms:LocationPeriodOrJurisdiction ;
.
dcterms:LCC
  a dcam:VocabularyEncodingScheme ;
  dcterms:hasVersion <http://dublincore.org/usage/terms/history/#LCC-003> ;
  dcterms:issued "2000-07-11" ;
  dcterms:modified "2008-01-14" ;
  rdfs:comment "The set of conceptual resources specified by the Library of Congress Classification."@en-US ;
  rdfs:isDefinedBy dcterms: ;
  rdfs:label "LCC"@en-US ;
  rdfs:seeAlso <http://lcweb.loc.gov/catdir/cpso/lcco/lcco.html> ;
.
dcterms:LCSH
  a dcam:VocabularyEncodingScheme ;
  dcterms:hasVersion <http://dublincore.org/usage/terms/history/#LCSH-003> ;
  dcterms:issued "2000-07-11" ;
  dcterms:modified "2008-01-14" ;
  rdfs:comment "The set of labeled concepts specified by the Library of Congress Subject Headings."@en-US ;
  rdfs:isDefinedBy dcterms: ;
  rdfs:label "LCSH"@en-US ;
.
dcterms:LicenseDocument
  a rdfs:Class ;
  dcterms:hasVersion <http://dublincore.org/usage/terms/history/#LicenseDocument-001> ;
  dcterms:issued "2008-01-14" ;
  rdfs:comment "A legal document giving official permission to do something with a Resource."@en-US ;
  rdfs:isDefinedBy dcterms: ;
  rdfs:label "License Document"@en-US ;
  rdfs:subClassOf dcterms:RightsStatement ;
.
dcterms:LinguisticSystem
  a rdfs:Class ;
  dcterms:description "Examples include written, spoken, sign, and computer languages."@en-US ;
  dcterms:hasVersion <http://dublincore.org/usage/terms/history/#LinguisticSystem-001> ;
  dcterms:issued "2008-01-14" ;
  rdfs:comment "A system of signs, symbols, sounds, gestures, or rules used in communication."@en-US ;
  rdfs:isDefinedBy dcterms: ;
  rdfs:label "Linguistic System"@en-US ;
.
dcterms:Location
  a rdfs:Class ;
  dcterms:hasVersion <http://dublincore.org/usage/terms/history/#Location-001> ;
  dcterms:issued "2008-01-14" ;
  rdfs:comment "A spatial region or named place."@en-US ;
  rdfs:isDefinedBy dcterms: ;
  rdfs:label "Location"@en-US ;
  rdfs:subClassOf dcterms:LocationPeriodOrJurisdiction ;
.
dcterms:LocationPeriodOrJurisdiction
  a rdfs:Class ;
  dcterms:hasVersion <http://dublincore.org/usage/terms/history/#LocationPeriodOrJurisdiction-001> ;
  dcterms:issued "2008-01-14" ;
  rdfs:comment "A location, period of time, or jurisdiction."@en-US ;
  rdfs:isDefinedBy dcterms: ;
  rdfs:label "Location, Period, or Jurisdiction"@en-US ;
.
dcterms:MESH
  a dcam:VocabularyEncodingScheme ;
  dcterms:hasVersion <http://dublincore.org/usage/terms/history/#MESH-003> ;
  dcterms:issued "2000-07-11" ;
  dcterms:modified "2008-01-14" ;
  rdfs:comment "The set of labeled concepts specified by the Medical Subject Headings."@en-US ;
  rdfs:isDefinedBy dcterms: ;
  rdfs:label "MeSH"@en-US ;
  rdfs:seeAlso <http://www.nlm.nih.gov/mesh/meshhome.html> ;
.
dcterms:MediaType
  a rdfs:Class ;
  dcterms:hasVersion <http://dublincore.org/usage/terms/history/#MediaType-001> ;
  dcterms:issued "2008-01-14" ;
  rdfs:comment "A file format or physical medium."@en-US ;
  rdfs:isDefinedBy dcterms: ;
  rdfs:label "Media Type"@en-US ;
  rdfs:subClassOf dcterms:MediaTypeOrExtent ;
.
dcterms:MediaTypeOrExtent
  a rdfs:Class ;
  dcterms:hasVersion <http://dublincore.org/usage/terms/history/#MediaTypeOrExtent-001> ;
  dcterms:issued "2008-01-14" ;
  rdfs:comment "A media type or extent."@en-US ;
  rdfs:isDefinedBy dcterms: ;
  rdfs:label "Media Type or Extent"@en-US ;
.
dcterms:MethodOfAccrual
  a rdfs:Class ;
  dcterms:hasVersion <http://dublincore.org/usage/terms/history/#MethodOfAccrual-001> ;
  dcterms:issued "2008-01-14" ;
  rdfs:comment "A method by which resources are added to a collection."@en-US ;
  rdfs:isDefinedBy dcterms: ;
  rdfs:label "Method of Accrual"@en-US ;
.
dcterms:MethodOfInstruction
  a rdfs:Class ;
  dcterms:hasVersion <http://dublincore.org/usage/terms/history/#MethodOfInstruction-001> ;
  dcterms:issued "2008-01-14" ;
  rdfs:comment "A process that is used to engender knowledge, attitudes, and skills."@en-US ;
  rdfs:isDefinedBy dcterms: ;
  rdfs:label "Method of Instruction"@en-US ;
.
dcterms:NLM
  a dcam:VocabularyEncodingScheme ;
  dcterms:hasVersion <http://dublincore.org/usage/terms/history/#NLM-002> ;
  dcterms:issued "2005-06-13" ;
  dcterms:modified "2008-01-14" ;
  rdfs:comment "The set of conceptual resources specified by the National Library of Medicine Classification."@en-US ;
  rdfs:isDefinedBy dcterms: ;
  rdfs:label "NLM"@en-US ;
  rdfs:seeAlso <http://wwwcf.nlm.nih.gov/class/> ;
.
dcterms:Period
  a rdfs:Datatype ;
  dcterms:hasVersion <http://dublincore.org/usage/terms/history/#Period-003> ;
  dcterms:issued "2000-07-11" ;
  dcterms:modified "2008-01-14" ;
  rdfs:comment "The set of time intervals defined by their limits according to the DCMI Period Encoding Scheme."@en-US ;
  rdfs:isDefinedBy dcterms: ;
  rdfs:label "DCMI Period"@en-US ;
  rdfs:seeAlso <http://dublincore.org/documents/dcmi-period/> ;
.
dcterms:PeriodOfTime
  a rdfs:Class ;
  dcterms:hasVersion <http://dublincore.org/usage/terms/history/#PeriodOfTime-001> ;
  dcterms:issued "2008-01-14" ;
  rdfs:comment "An interval of time that is named or defined by its start and end dates."@en-US ;
  rdfs:isDefinedBy dcterms: ;
  rdfs:label "Period of Time"@en-US ;
  rdfs:subClassOf dcterms:LocationPeriodOrJurisdiction ;
.
dcterms:PhysicalMedium
  a rdfs:Class ;
  dcterms:description "Examples include paper, canvas, or DVD."@en-US ;
  dcterms:hasVersion <http://dublincore.org/usage/terms/history/#PhysicalMedium-001> ;
  dcterms:issued "2008-01-14" ;
  rdfs:comment "A physical material or carrier."@en-US ;
  rdfs:isDefinedBy dcterms: ;
  rdfs:label "Physical Medium"@en-US ;
  rdfs:subClassOf dcterms:MediaType ;
.
dcterms:PhysicalResource
  a rdfs:Class ;
  dcterms:hasVersion <http://dublincore.org/usage/terms/history/#PhysicalResource-001> ;
  dcterms:issued "2008-01-14" ;
  rdfs:comment "A material thing."@en-US ;
  rdfs:isDefinedBy dcterms: ;
  rdfs:label "Physical Resource"@en-US ;
.
dcterms:Point
  a rdfs:Datatype ;
  dcterms:hasVersion <http://dublincore.org/usage/terms/history/#Point-003> ;
  dcterms:issued "2000-07-11" ;
  dcterms:modified "2008-01-14" ;
  rdfs:comment "The set of points in space defined by their geographic coordinates according to the DCMI Point Encoding Scheme."@en-US ;
  rdfs:isDefinedBy dcterms: ;
  rdfs:label "DCMI Point"@en-US ;
  rdfs:seeAlso <http://dublincore.org/documents/dcmi-point/> ;
.
dcterms:Policy
  a rdfs:Class ;
  dcterms:hasVersion <http://dublincore.org/usage/terms/history/#Policy-001> ;
  dcterms:issued "2008-01-14" ;
  rdfs:comment "A plan or course of action by an authority, intended to influence and determine decisions, actions, and other matters."@en-US ;
  rdfs:isDefinedBy dcterms: ;
  rdfs:label "Policy"@en-US ;
.
dcterms:ProvenanceStatement
  a rdfs:Class ;
  dcterms:hasVersion <http://dublincore.org/usage/terms/history/#ProvenanceStatement-001> ;
  dcterms:issued "2008-01-14" ;
  rdfs:comment "A statement of any changes in ownership and custody of a resource since its creation that are significant for its authenticity, integrity, and interpretation."@en-US ;
  rdfs:isDefinedBy dcterms: ;
  rdfs:label "Provenance Statement"@en-US ;
.
dcterms:RFC1766
  a rdfs:Datatype ;
  dcterms:hasVersion <http://dublincore.org/usage/terms/history/#RFC1766-003> ;
  dcterms:issued "2000-07-11" ;
  dcterms:modified "2008-01-14" ;
  rdfs:comment "The set of tags, constructed according to RFC 1766, for the identification of languages."@en-US ;
  rdfs:isDefinedBy dcterms: ;
  rdfs:label "RFC 1766"@en-US ;
  rdfs:seeAlso <http://www.ietf.org/rfc/rfc1766.txt> ;
.
dcterms:RFC3066
  a rdfs:Datatype ;
  dcterms:description "RFC 3066 has been obsoleted by RFC 4646."@en-US ;
  dcterms:hasVersion <http://dublincore.org/usage/terms/history/#RFC3066-002> ;
  dcterms:issued "2002-07-13" ;
  dcterms:modified "2008-01-14" ;
  rdfs:comment "The set of tags constructed according to RFC 3066 for the identification of languages."@en-US ;
  rdfs:isDefinedBy dcterms: ;
  rdfs:label "RFC 3066"@en-US ;
  rdfs:seeAlso <http://www.ietf.org/rfc/rfc3066.txt> ;
.
dcterms:RFC4646
  a rdfs:Datatype ;
  dcterms:description "RFC 4646 obsoletes RFC 3066."@en-US ;
  dcterms:hasVersion <http://dublincore.org/usage/terms/history/#RFC4646-001> ;
  dcterms:issued "2008-01-14" ;
  rdfs:comment "The set of tags constructed according to RFC 4646 for the identification of languages."@en-US ;
  rdfs:isDefinedBy dcterms: ;
  rdfs:label "RFC 4646"@en-US ;
  rdfs:seeAlso <http://www.ietf.org/rfc/rfc4646.txt> ;
.
dcterms:RFC5646
  a rdfs:Datatype ;
  dcterms:description "RFC 5646 obsoletes RFC 4646."@en-US ;
  dcterms:hasVersion <http://dublincore.org/usage/terms/history/#RFC5646-001> ;
  dcterms:issued "2010-10-11" ;
  rdfs:comment "The set of tags constructed according to RFC 5646 for the identification of languages."@en-US ;
  rdfs:isDefinedBy dcterms: ;
  rdfs:label "RFC 5646"@en-US ;
  rdfs:seeAlso <http://www.ietf.org/rfc/rfc5646.txt> ;
.
dcterms:RightsStatement
  a rdfs:Class ;
  dcterms:hasVersion <http://dublincore.org/usage/terms/history/#RightsStatement-001> ;
  dcterms:issued "2008-01-14" ;
  rdfs:comment "A statement about the intellectual property rights (IPR) held in or over a Resource, a legal document giving official permission to do something with a resource, or a statement about access rights."@en-US ;
  rdfs:isDefinedBy dcterms: ;
  rdfs:label "Rights Statement"@en-US ;
.
dcterms:SizeOrDuration
  a rdfs:Class ;
  dcterms:description "Examples include a number of pages, a specification of length, width, and breadth, or a period in hours, minutes, and seconds."@en-US ;
  dcterms:hasVersion <http://dublincore.org/usage/terms/history/#SizeOrDuration-001> ;
  dcterms:issued "2008-01-14" ;
  rdfs:comment "A dimension or extent, or a time taken to play or execute."@en-US ;
  rdfs:isDefinedBy dcterms: ;
  rdfs:label "Size or Duration"@en-US ;
  rdfs:subClassOf dcterms:MediaTypeOrExtent ;
.
dcterms:Standard
  a rdfs:Class ;
  dcterms:hasVersion <http://dublincore.org/usage/terms/history/#Standard-001> ;
  dcterms:issued "2008-01-14" ;
  rdfs:comment "A basis for comparison; a reference point against which other things can be evaluated."@en-US ;
  rdfs:isDefinedBy dcterms: ;
  rdfs:label "Standard"@en-US ;
.
dcterms:TGN
  a dcam:VocabularyEncodingScheme ;
  dcterms:hasVersion <http://dublincore.org/usage/terms/history/#TGN-003> ;
  dcterms:issued "2000-07-11" ;
  dcterms:modified "2008-01-14" ;
  rdfs:comment "The set of places specified by the Getty Thesaurus of Geographic Names."@en-US ;
  rdfs:isDefinedBy dcterms: ;
  rdfs:label "TGN"@en-US ;
  rdfs:seeAlso <http://www.getty.edu/research/tools/vocabulary/tgn/index.html> ;
.
dcterms:UDC
  a dcam:VocabularyEncodingScheme ;
  dcterms:hasVersion <http://dublincore.org/usage/terms/history/#UDC-003> ;
  dcterms:issued "2000-07-11" ;
  dcterms:modified "2008-01-14" ;
  rdfs:comment "The set of conceptual resources specified by the Universal Decimal Classification."@en-US ;
  rdfs:isDefinedBy dcterms: ;
  rdfs:label "UDC"@en-US ;
  rdfs:seeAlso <http://www.udcc.org/> ;
.
dcterms:URI
  a rdfs:Datatype ;
  dcterms:hasVersion <http://dublincore.org/usage/terms/history/#URI-003> ;
  dcterms:issued "2000-07-11" ;
  dcterms:modified "2008-01-14" ;
  rdfs:comment "The set of identifiers constructed according to the generic syntax for Uniform Resource Identifiers as specified by the Internet Engineering Task Force."@en-US ;
  rdfs:isDefinedBy dcterms: ;
  rdfs:label "URI"@en-US ;
  rdfs:seeAlso <http://www.ietf.org/rfc/rfc3986.txt> ;
.
dcterms:W3CDTF
  a rdfs:Datatype ;
  dcterms:hasVersion <http://dublincore.org/usage/terms/history/#W3CDTF-003> ;
  dcterms:issued "2000-07-11" ;
  dcterms:modified "2008-01-14" ;
  rdfs:comment "The set of dates and times constructed according to the W3C Date and Time Formats Specification."@en-US ;
  rdfs:isDefinedBy dcterms: ;
  rdfs:label "W3C-DTF"@en-US ;
  rdfs:seeAlso <http://www.w3.org/TR/NOTE-datetime> ;
.
dcterms:abstract
  a rdf:Property ;
  dcterms:hasVersion <http://dublincore.org/usage/terms/history/#abstract-003> ;
  dcterms:issued "2000-07-11" ;
  dcterms:modified "2008-01-14" ;
  rdfs:comment "A summary of the resource."@en-US ;
  rdfs:isDefinedBy dcterms: ;
  rdfs:label "Abstract"@en-US ;
  rdfs:subPropertyOf dc:description ;
  rdfs:subPropertyOf dcterms:description ;
.
dcterms:accessRights
  a rdf:Property ;
  dcterms:description "Access Rights may include information regarding access or restrictions based on privacy, security, or other policies."@en-US ;
  dcterms:hasVersion <http://dublincore.org/usage/terms/history/#accessRights-002> ;
  dcterms:issued "2003-02-15" ;
  dcterms:modified "2008-01-14" ;
  rdfs:comment "Information about who can access the resource or an indication of its security status."@en-US ;
  rdfs:isDefinedBy dcterms: ;
  rdfs:label "Access Rights"@en-US ;
  rdfs:range dcterms:RightsStatement ;
  rdfs:subPropertyOf dc:rights ;
  rdfs:subPropertyOf dcterms:rights ;
.
dcterms:accrualMethod
  a rdf:Property ;
  dcterms:hasVersion <http://dublincore.org/usage/terms/history/#accrualMethod-003> ;
  dcterms:issued "2005-06-13" ;
  dcterms:modified "2010-10-11" ;
  rdfs:comment "The method by which items are added to a collection."@en-US ;
  rdfs:domain <http://purl.org/dc/dcmitype/Collection> ;
  rdfs:isDefinedBy dcterms: ;
  rdfs:label "Accrual Method"@en-US ;
  rdfs:range dcterms:MethodOfAccrual ;
.
dcterms:accrualPeriodicity
  a rdf:Property ;
  dcterms:hasVersion <http://dublincore.org/usage/terms/history/#accrualPeriodicity-003> ;
  dcterms:issued "2005-06-13" ;
  dcterms:modified "2010-10-11" ;
  rdfs:comment "The frequency with which items are added to a collection."@en-US ;
  rdfs:domain <http://purl.org/dc/dcmitype/Collection> ;
  rdfs:isDefinedBy dcterms: ;
  rdfs:label "Accrual Periodicity"@en-US ;
  rdfs:range dcterms:Frequency ;
.
dcterms:accrualPolicy
  a rdf:Property ;
  dcterms:hasVersion <http://dublincore.org/usage/terms/history/#accrualPolicy-003> ;
  dcterms:issued "2005-06-13" ;
  dcterms:modified "2010-10-11" ;
  rdfs:comment "The policy governing the addition of items to a collection."@en-US ;
  rdfs:domain <http://purl.org/dc/dcmitype/Collection> ;
  rdfs:isDefinedBy dcterms: ;
  rdfs:label "Accrual Policy"@en-US ;
  rdfs:range dcterms:Policy ;
.
dcterms:alternative
  a rdf:Property ;
  dcterms:description "The distinction between titles and alternative titles is application-specific."@en-US ;
  dcterms:hasVersion <http://dublincore.org/usage/terms/history/#alternative-003> ;
  dcterms:issued "2000-07-11" ;
  dcterms:modified "2010-10-11" ;
  rdfs:comment "An alternative name for the resource."@en-US ;
  rdfs:isDefinedBy dcterms: ;
  rdfs:label "Alternative Title"@en-US ;
  rdfs:range rdfs:Literal ;
  rdfs:subPropertyOf dc:title ;
  rdfs:subPropertyOf dcterms:title ;
.
dcterms:audience
  a rdf:Property ;
  dcterms:hasVersion <http://dublincore.org/usage/terms/history/#audience-003> ;
  dcterms:issued "2001-05-21" ;
  dcterms:modified "2008-01-14" ;
  rdfs:comment "A class of entity for whom the resource is intended or useful."@en-US ;
  rdfs:isDefinedBy dcterms: ;
  rdfs:label "Audience"@en-US ;
  rdfs:range dcterms:AgentClass ;
.
dcterms:available
  a rdf:Property ;
  dcterms:hasVersion <http://dublincore.org/usage/terms/history/#available-003> ;
  dcterms:issued "2000-07-11" ;
  dcterms:modified "2008-01-14" ;
  rdfs:comment "Date (often a range) that the resource became or will become available."@en-US ;
  rdfs:isDefinedBy dcterms: ;
  rdfs:label "Date Available"@en-US ;
  rdfs:range rdfs:Literal ;
  rdfs:subPropertyOf dc:date ;
  rdfs:subPropertyOf dcterms:date ;
.
dcterms:bibliographicCitation
  a rdf:Property ;
  dcterms:description "Recommended practice is to include sufficient bibliographic detail to identify the resource as unambiguously as possible."@en-US ;
  dcterms:hasVersion <http://dublincore.org/usage/terms/history/#bibliographicCitation-002> ;
  dcterms:issued "2003-02-15" ;
  dcterms:modified "2008-01-14" ;
  rdfs:comment "A bibliographic reference for the resource."@en-US ;
  rdfs:domain dcterms:BibliographicResource ;
  rdfs:isDefinedBy dcterms: ;
  rdfs:label "Bibliographic Citation"@en-US ;
  rdfs:range rdfs:Literal ;
  rdfs:subPropertyOf dc:identifier ;
  rdfs:subPropertyOf dcterms:identifier ;
.
dcterms:conformsTo
  a rdf:Property ;
  dcterms:hasVersion <http://dublincore.org/usage/terms/history/#conformsTo-003> ;
  dcterms:issued "2001-05-21" ;
  dcterms:modified "2008-01-14" ;
  rdfs:comment "An established standard to which the described resource conforms."@en-US ;
  rdfs:isDefinedBy dcterms: ;
  rdfs:label "Conforms To"@en-US ;
  rdfs:range dcterms:Standard ;
  rdfs:subPropertyOf dc:relation ;
  rdfs:subPropertyOf dcterms:relation ;
.
dcterms:contributor
  a rdf:Property ;
  dcterms:description "Examples of a Contributor include a person, an organization, or a service."@en-US ;
  dcterms:hasVersion <http://dublincore.org/usage/terms/history/#contributorT-001> ;
  dcterms:issued "2008-01-14" ;
  dcterms:modified "2010-10-11" ;
  rdfs:comment "An entity responsible for making contributions to the resource."@en-US ;
  rdfs:isDefinedBy dcterms: ;
  rdfs:label "Contributor"@en-US ;
  rdfs:range dcterms:Agent ;
  rdfs:subPropertyOf dc:contributor ;
.
dcterms:coverage
  a rdf:Property ;
  dcterms:description "Spatial topic and spatial applicability may be a named place or a location specified by its geographic coordinates. Temporal topic may be a named period, date, or date range. A jurisdiction may be a named administrative entity or a geographic place to which the resource applies. Recommended best practice is to use a controlled vocabulary such as the Thesaurus of Geographic Names [TGN]. Where appropriate, named places or time periods can be used in preference to numeric identifiers such as sets of coordinates or date ranges."@en-US ;
  dcterms:hasVersion <http://dublincore.org/usage/terms/history/#coverageT-001> ;
  dcterms:issued "2008-01-14" ;
  dcterms:modified "2008-01-14" ;
  rdfs:comment "The spatial or temporal topic of the resource, the spatial applicability of the resource, or the jurisdiction under which the resource is relevant."@en-US ;
  rdfs:isDefinedBy dcterms: ;
  rdfs:label "Coverage"@en-US ;
  rdfs:range dcterms:LocationPeriodOrJurisdiction ;
  rdfs:subPropertyOf dc:coverage ;
.
dcterms:created
  a rdf:Property ;
  dcterms:hasVersion <http://dublincore.org/usage/terms/history/#created-003> ;
  dcterms:issued "2000-07-11" ;
  dcterms:modified "2008-01-14" ;
  rdfs:comment "Date of creation of the resource."@en-US ;
  rdfs:isDefinedBy dcterms: ;
  rdfs:label "Date Created"@en-US ;
  rdfs:range rdfs:Literal ;
  rdfs:subPropertyOf dc:date ;
  rdfs:subPropertyOf dcterms:date ;
.
dcterms:creator
  a rdf:Property ;
  dcterms:description "Examples of a Creator include a person, an organization, or a service."@en-US ;
  dcterms:hasVersion <http://dublincore.org/usage/terms/history/#creatorT-002> ;
  dcterms:issued "2008-01-14" ;
  dcterms:modified "2010-10-11" ;
  rdfs:comment "An entity primarily responsible for making the resource."@en-US ;
  rdfs:isDefinedBy dcterms: ;
  rdfs:label "Creator"@en-US ;
  rdfs:range dcterms:Agent ;
  rdfs:subPropertyOf dc:creator ;
  rdfs:subPropertyOf dcterms:contributor ;
  owl:equivalentProperty foaf:maker ;
.
dcterms:date
  a rdf:Property ;
  dcterms:description "Date may be used to express temporal information at any level of granularity.  Recommended best practice is to use an encoding scheme, such as the W3CDTF profile of ISO 8601 [W3CDTF]."@en-US ;
  dcterms:hasVersion <http://dublincore.org/usage/terms/history/#dateT-001> ;
  dcterms:issued "2008-01-14" ;
  dcterms:modified "2008-01-14" ;
  rdfs:comment "A point or period of time associated with an event in the lifecycle of the resource."@en-US ;
  rdfs:isDefinedBy dcterms: ;
  rdfs:label "Date"@en-US ;
  rdfs:range rdfs:Literal ;
  rdfs:subPropertyOf dc:date ;
.
dcterms:dateAccepted
  a rdf:Property ;
  dcterms:description "Examples of resources to which a Date Accepted may be relevant are a thesis (accepted by a university department) or an article (accepted by a journal)."@en-US ;
  dcterms:hasVersion <http://dublincore.org/usage/terms/history/#dateAccepted-002> ;
  dcterms:issued "2002-07-13" ;
  dcterms:modified "2008-01-14" ;
  rdfs:comment "Date of acceptance of the resource."@en-US ;
  rdfs:isDefinedBy dcterms: ;
  rdfs:label "Date Accepted"@en-US ;
  rdfs:range rdfs:Literal ;
  rdfs:subPropertyOf dc:date ;
  rdfs:subPropertyOf dcterms:date ;
.
dcterms:dateCopyrighted
  a rdf:Property ;
  dcterms:hasVersion <http://dublincore.org/usage/terms/history/#dateCopyrighted-002> ;
  dcterms:issued "2002-07-13" ;
  dcterms:modified "2008-01-14" ;
  rdfs:comment "Date of copyright."@en-US ;
  rdfs:isDefinedBy dcterms: ;
  rdfs:label "Date Copyrighted"@en-US ;
  rdfs:range rdfs:Literal ;
  rdfs:subPropertyOf dc:date ;
  rdfs:subPropertyOf dcterms:date ;
.
dcterms:dateSubmitted
  a rdf:Property ;
  dcterms:description "Examples of resources to which a Date Submitted may be relevant are a thesis (submitted to a university department) or an article (submitted to a journal)."@en-US ;
  dcterms:hasVersion <http://dublincore.org/usage/terms/history/#dateSubmitted-002> ;
  dcterms:issued "2002-07-13" ;
  dcterms:modified "2008-01-14" ;
  rdfs:comment "Date of submission of the resource."@en-US ;
  rdfs:isDefinedBy dcterms: ;
  rdfs:label "Date Submitted"@en-US ;
  rdfs:range rdfs:Literal ;
  rdfs:subPropertyOf dc:date ;
  rdfs:subPropertyOf dcterms:date ;
.
dcterms:description
  a rdf:Property ;
  dcterms:description "Description may include but is not limited to: an abstract, a table of contents, a graphical representation, or a free-text account of the resource."@en-US ;
  dcterms:hasVersion <http://dublincore.org/usage/terms/history/#descriptionT-001> ;
  dcterms:issued "2008-01-14" ;
  dcterms:modified "2008-01-14" ;
  rdfs:comment "An account of the resource."@en-US ;
  rdfs:isDefinedBy dcterms: ;
  rdfs:label "Description"@en-US ;
  rdfs:subPropertyOf dc:description ;
.
dcterms:educationLevel
  a rdf:Property ;
  dcterms:hasVersion <http://dublincore.org/usage/terms/history/#educationLevel-002> ;
  dcterms:issued "2002-07-13" ;
  dcterms:modified "2008-01-14" ;
  rdfs:comment "A class of entity, defined in terms of progression through an educational or training context, for which the described resource is intended."@en-US ;
  rdfs:isDefinedBy dcterms: ;
  rdfs:label "Audience Education Level"@en-US ;
  rdfs:range dcterms:AgentClass ;
  rdfs:subPropertyOf dcterms:audience ;
.
dcterms:extent
  a rdf:Property ;
  dcterms:hasVersion <http://dublincore.org/usage/terms/history/#extent-003> ;
  dcterms:issued "2000-07-11" ;
  dcterms:modified "2008-01-14" ;
  rdfs:comment "The size or duration of the resource."@en-US ;
  rdfs:isDefinedBy dcterms: ;
  rdfs:label "Extent"@en-US ;
  rdfs:range dcterms:SizeOrDuration ;
  rdfs:subPropertyOf dc:format ;
  rdfs:subPropertyOf dcterms:format ;
.
dcterms:format
  a rdf:Property ;
  dcterms:description "Examples of dimensions include size and duration. Recommended best practice is to use a controlled vocabulary such as the list of Internet Media Types [MIME]."@en-US ;
  dcterms:hasVersion <http://dublincore.org/usage/terms/history/#formatT-001> ;
  dcterms:issued "2008-01-14" ;
  dcterms:modified "2008-01-14" ;
  rdfs:comment "The file format, physical medium, or dimensions of the resource."@en-US ;
  rdfs:isDefinedBy dcterms: ;
  rdfs:label "Format"@en-US ;
  rdfs:range dcterms:MediaTypeOrExtent ;
  rdfs:subPropertyOf dc:format ;
.
dcterms:hasFormat
  a rdf:Property ;
  dcterms:hasVersion <http://dublincore.org/usage/terms/history/#hasFormat-003> ;
  dcterms:issued "2000-07-11" ;
  dcterms:modified "2008-01-14" ;
  rdfs:comment "A related resource that is substantially the same as the pre-existing described resource, but in another format."@en-US ;
  rdfs:isDefinedBy dcterms: ;
  rdfs:label "Has Format"@en-US ;
  rdfs:subPropertyOf dc:relation ;
  rdfs:subPropertyOf dcterms:relation ;
  skos:note "This term is intended to be used with non-literal values as defined in the DCMI Abstract Model (http://dublincore.org/documents/abstract-model/).  As of December 2007, the DCMI Usage Board is seeking a way to express this intention with a formal range declaration."@en-US ;
.
dcterms:hasPart
  a rdf:Property ;
  dcterms:hasVersion <http://dublincore.org/usage/terms/history/#hasPart-003> ;
  dcterms:issued "2000-07-11" ;
  dcterms:modified "2008-01-14" ;
  rdfs:comment "A related resource that is included either physically or logically in the described resource."@en-US ;
  rdfs:isDefinedBy dcterms: ;
  rdfs:label "Has Part"@en-US ;
  rdfs:subPropertyOf dc:relation ;
  rdfs:subPropertyOf dcterms:relation ;
  skos:note "This term is intended to be used with non-literal values as defined in the DCMI Abstract Model (http://dublincore.org/documents/abstract-model/).  As of December 2007, the DCMI Usage Board is seeking a way to express this intention with a formal range declaration."@en-US ;
.
dcterms:hasVersion
  a rdf:Property ;
  dcterms:hasVersion <http://dublincore.org/usage/terms/history/#hasVersion-003> ;
  dcterms:issued "2000-07-11" ;
  dcterms:modified "2008-01-14" ;
  rdfs:comment "A related resource that is a version, edition, or adaptation of the described resource."@en-US ;
  rdfs:isDefinedBy dcterms: ;
  rdfs:label "Has Version"@en-US ;
  rdfs:subPropertyOf dc:relation ;
  rdfs:subPropertyOf dcterms:relation ;
  skos:note "This term is intended to be used with non-literal values as defined in the DCMI Abstract Model (http://dublincore.org/documents/abstract-model/).  As of December 2007, the DCMI Usage Board is seeking a way to express this intention with a formal range declaration."@en-US ;
.
dcterms:identifier
  a rdf:Property ;
  dcterms:description "Recommended best practice is to identify the resource by means of a string conforming to a formal identification system. "@en-US ;
  dcterms:hasVersion <http://dublincore.org/usage/terms/history/#identifierT-001> ;
  dcterms:issued "2008-01-14" ;
  dcterms:modified "2008-01-14" ;
  rdfs:comment "An unambiguous reference to the resource within a given context."@en-US ;
  rdfs:isDefinedBy dcterms: ;
  rdfs:label "Identifier"@en-US ;
  rdfs:range rdfs:Literal ;
  rdfs:subPropertyOf dc:identifier ;
.
dcterms:instructionalMethod
  a rdf:Property ;
  dcterms:description "Instructional Method will typically include ways of presenting instructional materials or conducting instructional activities, patterns of learner-to-learner and learner-to-instructor interactions, and mechanisms by which group and individual levels of learning are measured.  Instructional methods include all aspects of the instruction and learning processes from planning and implementation through evaluation and feedback."@en-US ;
  dcterms:hasVersion <http://dublincore.org/usage/terms/history/#instructionalMethod-002> ;
  dcterms:issued "2005-06-13" ;
  dcterms:modified "2008-01-14" ;
  rdfs:comment "A process, used to engender knowledge, attitudes and skills, that the described resource is designed to support."@en-US ;
  rdfs:isDefinedBy dcterms: ;
  rdfs:label "Instructional Method"@en-US ;
  rdfs:range dcterms:MethodOfInstruction ;
.
dcterms:isFormatOf
  a rdf:Property ;
  dcterms:hasVersion <http://dublincore.org/usage/terms/history/#isFormatOf-003> ;
  dcterms:issued "2000-07-11" ;
  dcterms:modified "2008-01-14" ;
  rdfs:comment "A related resource that is substantially the same as the described resource, but in another format."@en-US ;
  rdfs:isDefinedBy dcterms: ;
  rdfs:label "Is Format Of"@en-US ;
  rdfs:subPropertyOf dc:relation ;
  rdfs:subPropertyOf dcterms:relation ;
  skos:note "This term is intended to be used with non-literal values as defined in the DCMI Abstract Model (http://dublincore.org/documents/abstract-model/).  As of December 2007, the DCMI Usage Board is seeking a way to express this intention with a formal range declaration."@en-US ;
.
dcterms:isPartOf
  a rdf:Property ;
  dcterms:hasVersion <http://dublincore.org/usage/terms/history/#isPartOf-003> ;
  dcterms:issued "2000-07-11" ;
  dcterms:modified "2008-01-14" ;
  rdfs:comment "A related resource in which the described resource is physically or logically included."@en-US ;
  rdfs:isDefinedBy dcterms: ;
  rdfs:label "Is Part Of"@en-US ;
  rdfs:subPropertyOf dc:relation ;
  rdfs:subPropertyOf dcterms:relation ;
  skos:note "This term is intended to be used with non-literal values as defined in the DCMI Abstract Model (http://dublincore.org/documents/abstract-model/).  As of December 2007, the DCMI Usage Board is seeking a way to express this intention with a formal range declaration."@en-US ;
.
dcterms:isReferencedBy
  a rdf:Property ;
  dcterms:hasVersion <http://dublincore.org/usage/terms/history/#isReferencedBy-003> ;
  dcterms:issued "2000-07-11" ;
  dcterms:modified "2008-01-14" ;
  rdfs:comment "A related resource that references, cites, or otherwise points to the described resource."@en-US ;
  rdfs:isDefinedBy dcterms: ;
  rdfs:label "Is Referenced By"@en-US ;
  rdfs:subPropertyOf dc:relation ;
  rdfs:subPropertyOf dcterms:relation ;
  skos:note "This term is intended to be used with non-literal values as defined in the DCMI Abstract Model (http://dublincore.org/documents/abstract-model/).  As of December 2007, the DCMI Usage Board is seeking a way to express this intention with a formal range declaration."@en-US ;
.
dcterms:isReplacedBy
  a rdf:Property ;
  dcterms:hasVersion <http://dublincore.org/usage/terms/history/#isReplacedBy-003> ;
  dcterms:issued "2000-07-11" ;
  dcterms:modified "2008-01-14" ;
  rdfs:comment "A related resource that supplants, displaces, or supersedes the described resource."@en-US ;
  rdfs:isDefinedBy dcterms: ;
  rdfs:label "Is Replaced By"@en-US ;
  rdfs:subPropertyOf dc:relation ;
  rdfs:subPropertyOf dcterms:relation ;
  skos:note "This term is intended to be used with non-literal values as defined in the DCMI Abstract Model (http://dublincore.org/documents/abstract-model/).  As of December 2007, the DCMI Usage Board is seeking a way to express this intention with a formal range declaration."@en-US ;
.
dcterms:isRequiredBy
  a rdf:Property ;
  dcterms:hasVersion <http://dublincore.org/usage/terms/history/#isRequiredBy-003> ;
  dcterms:issued "2000-07-11" ;
  dcterms:modified "2008-01-14" ;
  rdfs:comment "A related resource that requires the described resource to support its function, delivery, or coherence."@en-US ;
  rdfs:isDefinedBy dcterms: ;
  rdfs:label "Is Required By"@en-US ;
  rdfs:subPropertyOf dc:relation ;
  rdfs:subPropertyOf dcterms:relation ;
  skos:note "This term is intended to be used with non-literal values as defined in the DCMI Abstract Model (http://dublincore.org/documents/abstract-model/).  As of December 2007, the DCMI Usage Board is seeking a way to express this intention with a formal range declaration."@en-US ;
.
dcterms:isVersionOf
  a rdf:Property ;
  dcterms:description "Changes in version imply substantive changes in content rather than differences in format."@en-US ;
  dcterms:hasVersion <http://dublincore.org/usage/terms/history/#isVersionOf-003> ;
  dcterms:issued "2000-07-11" ;
  dcterms:modified "2008-01-14" ;
  rdfs:comment "A related resource of which the described resource is a version, edition, or adaptation."@en-US ;
  rdfs:isDefinedBy dcterms: ;
  rdfs:label "Is Version Of"@en-US ;
  rdfs:subPropertyOf dc:relation ;
  rdfs:subPropertyOf dcterms:relation ;
  skos:note "This term is intended to be used with non-literal values as defined in the DCMI Abstract Model (http://dublincore.org/documents/abstract-model/).  As of December 2007, the DCMI Usage Board is seeking a way to express this intention with a formal range declaration."@en-US ;
.
dcterms:issued
  a rdf:Property ;
  dcterms:hasVersion <http://dublincore.org/usage/terms/history/#issued-003> ;
  dcterms:issued "2000-07-11" ;
  dcterms:modified "2008-01-14" ;
  rdfs:comment "Date of formal issuance (e.g., publication) of the resource."@en-US ;
  rdfs:isDefinedBy dcterms: ;
  rdfs:label "Date Issued"@en-US ;
  rdfs:range rdfs:Literal ;
  rdfs:subPropertyOf dc:date ;
  rdfs:subPropertyOf dcterms:date ;
.
dcterms:language
  a rdf:Property ;
  dcterms:description "Recommended best practice is to use a controlled vocabulary such as RFC 4646 [RFC4646]."@en-US ;
  dcterms:hasVersion <http://dublincore.org/usage/terms/history/#languageT-001> ;
  dcterms:issued "2008-01-14" ;
  dcterms:modified "2008-01-14" ;
  rdfs:comment "A language of the resource."@en-US ;
  rdfs:isDefinedBy dcterms: ;
  rdfs:label "Language"@en-US ;
  rdfs:range dcterms:LinguisticSystem ;
  rdfs:subPropertyOf dc:language ;
.
dcterms:license
  a rdf:Property ;
  dcterms:hasVersion <http://dublincore.org/usage/terms/history/#license-002> ;
  dcterms:issued "2004-06-14" ;
  dcterms:modified "2008-01-14" ;
  rdfs:comment "A legal document giving official permission to do something with the resource."@en-US ;
  rdfs:isDefinedBy dcterms: ;
  rdfs:label "License"@en-US ;
  rdfs:range dcterms:LicenseDocument ;
  rdfs:subPropertyOf dc:rights ;
  rdfs:subPropertyOf dcterms:rights ;
.
dcterms:mediator
  a rdf:Property ;
  dcterms:description "In an educational context, a mediator might be a parent, teacher, teaching assistant, or care-giver."@en-US ;
  dcterms:hasVersion <http://dublincore.org/usage/terms/history/#mediator-003> ;
  dcterms:issued "2001-05-21" ;
  dcterms:modified "2008-01-14" ;
  rdfs:comment "An entity that mediates access to the resource and for whom the resource is intended or useful."@en-US ;
  rdfs:isDefinedBy dcterms: ;
  rdfs:label "Mediator"@en-US ;
  rdfs:range dcterms:AgentClass ;
  rdfs:subPropertyOf dcterms:audience ;
.
dcterms:medium
  a rdf:Property ;
  dcterms:hasVersion <http://dublincore.org/usage/terms/history/#medium-003> ;
  dcterms:issued "2000-07-11" ;
  dcterms:modified "2008-01-14" ;
  rdfs:comment "The material or physical carrier of the resource."@en-US ;
  rdfs:domain dcterms:PhysicalResource ;
  rdfs:isDefinedBy dcterms: ;
  rdfs:label "Medium"@en-US ;
  rdfs:range dcterms:PhysicalMedium ;
  rdfs:subPropertyOf dc:format ;
  rdfs:subPropertyOf dcterms:format ;
.
dcterms:modified
  a rdf:Property ;
  dcterms:hasVersion <http://dublincore.org/usage/terms/history/#modified-003> ;
  dcterms:issued "2000-07-11" ;
  dcterms:modified "2008-01-14" ;
  rdfs:comment "Date on which the resource was changed."@en-US ;
  rdfs:isDefinedBy dcterms: ;
  rdfs:label "Date Modified"@en-US ;
  rdfs:range rdfs:Literal ;
  rdfs:subPropertyOf dc:date ;
  rdfs:subPropertyOf dcterms:date ;
.
dcterms:provenance
  a rdf:Property ;
  dcterms:description "The statement may include a description of any changes successive custodians made to the resource."@en-US ;
  dcterms:hasVersion <http://dublincore.org/usage/terms/history/#provenance-002> ;
  dcterms:issued "2004-09-20" ;
  dcterms:modified "2008-01-14" ;
  rdfs:comment "A statement of any changes in ownership and custody of the resource since its creation that are significant for its authenticity, integrity, and interpretation."@en-US ;
  rdfs:isDefinedBy dcterms: ;
  rdfs:label "Provenance"@en-US ;
  rdfs:range dcterms:ProvenanceStatement ;
.
dcterms:publisher
  a rdf:Property ;
  dcterms:description "Examples of a Publisher include a person, an organization, or a service."@en-US ;
  dcterms:hasVersion <http://dublincore.org/usage/terms/history/#publisherT-001> ;
  dcterms:issued "2008-01-14" ;
  dcterms:modified "2010-10-11" ;
  rdfs:comment "An entity responsible for making the resource available."@en-US ;
  rdfs:isDefinedBy dcterms: ;
  rdfs:label "Publisher"@en-US ;
  rdfs:range dcterms:Agent ;
  rdfs:subPropertyOf dc:publisher ;
.
dcterms:references
  a rdf:Property ;
  dcterms:hasVersion <http://dublincore.org/usage/terms/history/#references-003> ;
  dcterms:issued "2000-07-11" ;
  dcterms:modified "2008-01-14" ;
  rdfs:comment "A related resource that is referenced, cited, or otherwise pointed to by the described resource."@en-US ;
  rdfs:isDefinedBy dcterms: ;
  rdfs:label "References"@en-US ;
  rdfs:subPropertyOf dc:relation ;
  rdfs:subPropertyOf dcterms:relation ;
  skos:note "This term is intended to be used with non-literal values as defined in the DCMI Abstract Model (http://dublincore.org/documents/abstract-model/).  As of December 2007, the DCMI Usage Board is seeking a way to express this intention with a formal range declaration."@en-US ;
.
dcterms:relation
  a rdf:Property ;
  dcterms:description "Recommended best practice is to identify the related resource by means of a string conforming to a formal identification system. "@en-US ;
  dcterms:hasVersion <http://dublincore.org/usage/terms/history/#relationT-001> ;
  dcterms:issued "2008-01-14" ;
  dcterms:modified "2008-01-14" ;
  rdfs:comment "A related resource."@en-US ;
  rdfs:isDefinedBy dcterms: ;
  rdfs:label "Relation"@en-US ;
  rdfs:subPropertyOf dc:relation ;
  skos:note "This term is intended to be used with non-literal values as defined in the DCMI Abstract Model (http://dublincore.org/documents/abstract-model/).  As of December 2007, the DCMI Usage Board is seeking a way to express this intention with a formal range declaration."@en-US ;
.
dcterms:replaces
  a rdf:Property ;
  dcterms:hasVersion <http://dublincore.org/usage/terms/history/#replaces-003> ;
  dcterms:issued "2000-07-11" ;
  dcterms:modified "2008-01-14" ;
  rdfs:comment "A related resource that is supplanted, displaced, or superseded by the described resource."@en-US ;
  rdfs:isDefinedBy dcterms: ;
  rdfs:label "Replaces"@en-US ;
  rdfs:subPropertyOf dc:relation ;
  rdfs:subPropertyOf dcterms:relation ;
  skos:note "This term is intended to be used with non-literal values as defined in the DCMI Abstract Model (http://dublincore.org/documents/abstract-model/).  As of December 2007, the DCMI Usage Board is seeking a way to express this intention with a formal range declaration."@en-US ;
.
dcterms:requires
  a rdf:Property ;
  dcterms:hasVersion <http://dublincore.org/usage/terms/history/#requires-003> ;
  dcterms:issued "2000-07-11" ;
  dcterms:modified "2008-01-14" ;
  rdfs:comment "A related resource that is required by the described resource to support its function, delivery, or coherence."@en-US ;
  rdfs:isDefinedBy dcterms: ;
  rdfs:label "Requires"@en-US ;
  rdfs:subPropertyOf dc:relation ;
  rdfs:subPropertyOf dcterms:relation ;
  skos:note "This term is intended to be used with non-literal values as defined in the DCMI Abstract Model (http://dublincore.org/documents/abstract-model/).  As of December 2007, the DCMI Usage Board is seeking a way to express this intention with a formal range declaration."@en-US ;
.
dcterms:rights
  a rdf:Property ;
  dcterms:description "Typically, rights information includes a statement about various property rights associated with the resource, including intellectual property rights."@en-US ;
  dcterms:hasVersion <http://dublincore.org/usage/terms/history/#rightsT-001> ;
  dcterms:issued "2008-01-14" ;
  dcterms:modified "2008-01-14" ;
  rdfs:comment "Information about rights held in and over the resource."@en-US ;
  rdfs:isDefinedBy dcterms: ;
  rdfs:label "Rights"@en-US ;
  rdfs:range dcterms:RightsStatement ;
  rdfs:subPropertyOf dc:rights ;
.
dcterms:rightsHolder
  a rdf:Property ;
  dcterms:hasVersion <http://dublincore.org/usage/terms/history/#rightsHolder-002> ;
  dcterms:issued "2004-06-14" ;
  dcterms:modified "2008-01-14" ;
  rdfs:comment "A person or organization owning or managing rights over the resource."@en-US ;
  rdfs:isDefinedBy dcterms: ;
  rdfs:label "Rights Holder"@en-US ;
  rdfs:range dcterms:Agent ;
.
dcterms:source
  a rdf:Property ;
  dcterms:description "The described resource may be derived from the related resource in whole or in part. Recommended best practice is to identify the related resource by means of a string conforming to a formal identification system."@en-US ;
  dcterms:hasVersion <http://dublincore.org/usage/terms/history/#sourceT-001> ;
  dcterms:issued "2008-01-14" ;
  dcterms:modified "2008-01-14" ;
  rdfs:comment "A related resource from which the described resource is derived."@en-US ;
  rdfs:isDefinedBy dcterms: ;
  rdfs:label "Source"@en-US ;
  rdfs:subPropertyOf dc:source ;
  rdfs:subPropertyOf dcterms:relation ;
  skos:note "This term is intended to be used with non-literal values as defined in the DCMI Abstract Model (http://dublincore.org/documents/abstract-model/).  As of December 2007, the DCMI Usage Board is seeking a way to express this intention with a formal range declaration."@en-US ;
.
dcterms:spatial
  a rdf:Property ;
  dcterms:hasVersion <http://dublincore.org/usage/terms/history/#spatial-003> ;
  dcterms:issued "2000-07-11" ;
  dcterms:modified "2008-01-14" ;
  rdfs:comment "Spatial characteristics of the resource."@en-US ;
  rdfs:isDefinedBy dcterms: ;
  rdfs:label "Spatial Coverage"@en-US ;
  rdfs:range dcterms:Location ;
  rdfs:subPropertyOf dc:coverage ;
  rdfs:subPropertyOf dcterms:coverage ;
.
dcterms:subject
  a rdf:Property ;
  dcterms:description "Typically, the subject will be represented using keywords, key phrases, or classification codes. Recommended best practice is to use a controlled vocabulary. To describe the spatial or temporal topic of the resource, use the Coverage element."@en-US ;
  dcterms:hasVersion <http://dublincore.org/usage/terms/history/#subjectT-001> ;
  dcterms:issued "2008-01-14" ;
  dcterms:modified "2008-01-14" ;
  rdfs:comment "The topic of the resource."@en-US ;
  rdfs:isDefinedBy dcterms: ;
  rdfs:label "Subject"@en-US ;
  rdfs:subPropertyOf dc:subject ;
  skos:note "This term is intended to be used with non-literal values as defined in the DCMI Abstract Model (http://dublincore.org/documents/abstract-model/).  As of December 2007, the DCMI Usage Board is seeking a way to express this intention with a formal range declaration."@en-US ;
.
dcterms:tableOfContents
  a rdf:Property ;
  dcterms:hasVersion <http://dublincore.org/usage/terms/history/#tableOfContents-003> ;
  dcterms:issued "2000-07-11" ;
  dcterms:modified "2008-01-14" ;
  rdfs:comment "A list of subunits of the resource."@en-US ;
  rdfs:isDefinedBy dcterms: ;
  rdfs:label "Table Of Contents"@en-US ;
  rdfs:subPropertyOf dc:description ;
  rdfs:subPropertyOf dcterms:description ;
.
dcterms:temporal
  a rdf:Property ;
  dcterms:hasVersion <http://dublincore.org/usage/terms/history/#temporal-003> ;
  dcterms:issued "2000-07-11" ;
  dcterms:modified "2008-01-14" ;
  rdfs:comment "Temporal characteristics of the resource."@en-US ;
  rdfs:isDefinedBy dcterms: ;
  rdfs:label "Temporal Coverage"@en-US ;
  rdfs:range dcterms:PeriodOfTime ;
  rdfs:subPropertyOf dc:coverage ;
  rdfs:subPropertyOf dcterms:coverage ;
.
dcterms:title
  a rdf:Property ;
  dcterms:hasVersion <http://dublincore.org/usage/terms/history/#titleT-002> ;
  dcterms:issued "2008-01-14" ;
  dcterms:modified "2010-10-11" ;
  rdfs:comment "A name given to the resource."@en-US ;
  rdfs:isDefinedBy dcterms: ;
  rdfs:label "Title"@en-US ;
  rdfs:range rdfs:Literal ;
  rdfs:subPropertyOf dc:title ;
.
dcterms:type
  a rdf:Property ;
  dcterms:description "Recommended best practice is to use a controlled vocabulary such as the DCMI Type Vocabulary [DCMITYPE]. To describe the file format, physical medium, or dimensions of the resource, use the Format element."@en-US ;
  dcterms:hasVersion <http://dublincore.org/usage/terms/history/#typeT-001> ;
  dcterms:issued "2008-01-14" ;
  dcterms:modified "2008-01-14" ;
  rdfs:comment "The nature or genre of the resource."@en-US ;
  rdfs:isDefinedBy dcterms: ;
  rdfs:label "Type"@en-US ;
  rdfs:range rdfs:Class ;
  rdfs:subPropertyOf dc:type ;
.
dcterms:valid
  a rdf:Property ;
  dcterms:hasVersion <http://dublincore.org/usage/terms/history/#valid-003> ;
  dcterms:issued "2000-07-11" ;
  dcterms:modified "2008-01-14" ;
  rdfs:comment "Date (often a range) of validity of a resource."@en-US ;
  rdfs:isDefinedBy dcterms: ;
  rdfs:label "Date Valid"@en-US ;
  rdfs:range rdfs:Literal ;
  rdfs:subPropertyOf dc:date ;
  rdfs:subPropertyOf dcterms:date ;
.
<http://www.w3.org/2004/02/skos/core>
  dcterms:contributor "Dave Beckett" ;
  dcterms:contributor "Nikki Rogers" ;
  dcterms:contributor "Participants in W3C's Semantic Web Deployment Working Group." ;
  dcterms:creator "Alistair Miles" ;
  dcterms:creator "Sean Bechhofer" ;
  dcterms:description "An RDF vocabulary for describing the basic structure and content of concept schemes such as thesauri, classification schemes, subject heading lists, taxonomies, 'folksonomies', other types of controlled vocabulary, and also concept schemes embedded in glossaries and terminologies."@en ;
  dcterms:title "SKOS Vocabulary"@en ;
  rdfs:label "SKOS Core RDF vocabulary" ;
  rdfs:seeAlso <http://www.w3.org/TR/skos-reference/> ;
  owl:versionInfo "Modified by TopQuadrant to assert three rdfs:subClassOf owl:Thing triples." ;
.
skos:Collection
  a owl:Class ;
  rdfs:isDefinedBy <http://www.w3.org/2004/02/skos/core> ;
  rdfs:label "Collection"@en ;
  rdfs:subClassOf owl:Thing ;
  owl:disjointWith skos:Concept ;
  owl:disjointWith skos:ConceptScheme ;
  skos:definition "A meaningful collection of concepts."@en ;
  skos:scopeNote "Labelled collections can be used where you would like a set of concepts to be displayed under a 'node label' in the hierarchy."@en ;
.
skos:Concept
  a owl:Class ;
  rdfs:isDefinedBy <http://www.w3.org/2004/02/skos/core> ;
  rdfs:label "Concept"@en ;
  rdfs:subClassOf owl:Thing ;
  skos:definition "An idea or notion; a unit of thought."@en ;
.
skos:ConceptScheme
  a owl:Class ;
  rdfs:isDefinedBy <http://www.w3.org/2004/02/skos/core> ;
  rdfs:label "Concept Scheme"@en ;
  rdfs:subClassOf owl:Thing ;
  owl:disjointWith skos:Concept ;
  skos:definition "A set of concepts, optionally including statements about semantic relationships between those concepts."@en ;
  skos:example "Thesauri, classification schemes, subject heading lists, taxonomies, 'folksonomies', and other types of controlled vocabulary are all examples of concept schemes. Concept schemes are also embedded in glossaries and terminologies."@en ;
  skos:scopeNote "A concept scheme may be defined to include concepts from different sources."@en ;
.
skos:OrderedCollection
  a owl:Class ;
  rdfs:isDefinedBy <http://www.w3.org/2004/02/skos/core> ;
  rdfs:label "Ordered Collection"@en ;
  rdfs:subClassOf skos:Collection ;
  skos:definition "An ordered collection of concepts, where both the grouping and the ordering are meaningful."@en ;
  skos:scopeNote "Ordered collections can be used where you would like a set of concepts to be displayed in a specific order, and optionally under a 'node label'."@en ;
.
skos:altLabel
  a rdf:Property ;
  a owl:AnnotationProperty ;
  rdfs:comment "The range of skos:altLabel is the class of RDF plain literals."@en ;
  rdfs:comment "skos:prefLabel, skos:altLabel and skos:hiddenLabel are pairwise disjoint properties."@en ;
  rdfs:isDefinedBy <http://www.w3.org/2004/02/skos/core> ;
  rdfs:label "alternative label"@en ;
  rdfs:subPropertyOf rdfs:label ;
  skos:definition "An alternative lexical label for a resource."@en ;
  skos:example "Acronyms, abbreviations, spelling variants, and irregular plural/singular forms may be included among the alternative labels for a concept. Mis-spelled terms are normally included as hidden labels (see skos:hiddenLabel)."@en ;
.
skos:broadMatch
  a rdf:Property ;
  a owl:ObjectProperty ;
  rdfs:isDefinedBy <http://www.w3.org/2004/02/skos/core> ;
  rdfs:label "has broader match"@en ;
  rdfs:subPropertyOf skos:broader ;
  rdfs:subPropertyOf skos:mappingRelation ;
  owl:inverseOf skos:narrowMatch ;
  skos:definition "skos:broadMatch is used to state a hierarchical mapping link between two conceptual resources in different concept schemes."@en ;
.
skos:broader
  a rdf:Property ;
  a owl:ObjectProperty ;
  rdfs:comment "Broader concepts are typically rendered as parents in a concept hierarchy (tree)."@en ;
  rdfs:isDefinedBy <http://www.w3.org/2004/02/skos/core> ;
  rdfs:label "has broader"@en ;
  rdfs:subPropertyOf skos:broaderTransitive ;
  owl:inverseOf skos:narrower ;
  skos:definition "Relates a concept to a concept that is more general in meaning."@en ;
  skos:scopeNote "By convention, skos:broader is only used to assert an immediate (i.e. direct) hierarchical link between two conceptual resources."@en ;
.
skos:broaderTransitive
  a rdf:Property ;
  a owl:ObjectProperty ;
  a owl:TransitiveProperty ;
  rdfs:isDefinedBy <http://www.w3.org/2004/02/skos/core> ;
  rdfs:label "has broader transitive"@en ;
  rdfs:subPropertyOf skos:semanticRelation ;
  owl:inverseOf skos:narrowerTransitive ;
  skos:definition "skos:broaderTransitive is a transitive superproperty of skos:broader." ;
  skos:scopeNote "By convention, skos:broaderTransitive is not used to make assertions. Rather, the properties can be used to draw inferences about the transitive closure of the hierarchical relation, which is useful e.g. when implementing a simple query expansion algorithm in a search application."@en ;
.
skos:changeNote
  a rdf:Property ;
  a owl:AnnotationProperty ;
  rdfs:isDefinedBy <http://www.w3.org/2004/02/skos/core> ;
  rdfs:label "change note"@en ;
  rdfs:subPropertyOf skos:note ;
  skos:definition "A note about a modification to a concept."@en ;
.
skos:closeMatch
  a rdf:Property ;
  a owl:ObjectProperty ;
  a owl:SymmetricProperty ;
  rdfs:isDefinedBy <http://www.w3.org/2004/02/skos/core> ;
  rdfs:label "has close match"@en ;
  rdfs:subPropertyOf skos:mappingRelation ;
  skos:definition "skos:closeMatch is used to link two concepts that are sufficiently similar that they can be used interchangeably in some information retrieval applications. In order to avoid the possibility of \"compound errors\" when combining mappings across more than two concept schemes, skos:closeMatch is not declared to be a transitive property."@en ;
.
skos:definition
  a rdf:Property ;
  a owl:AnnotationProperty ;
  rdfs:isDefinedBy <http://www.w3.org/2004/02/skos/core> ;
  rdfs:label "definition"@en ;
  rdfs:subPropertyOf skos:note ;
  skos:definition "A statement or formal explanation of the meaning of a concept."@en ;
.
skos:editorialNote
  a rdf:Property ;
  a owl:AnnotationProperty ;
  rdfs:isDefinedBy <http://www.w3.org/2004/02/skos/core> ;
  rdfs:label "editorial note"@en ;
  rdfs:subPropertyOf skos:note ;
  skos:definition "A note for an editor, translator or maintainer of the vocabulary."@en ;
.
skos:exactMatch
  a rdf:Property ;
  a owl:ObjectProperty ;
  a owl:SymmetricProperty ;
  a owl:TransitiveProperty ;
  rdfs:comment "skos:exactMatch is disjoint with each of the properties skos:broadMatch and skos:relatedMatch."@en ;
  rdfs:isDefinedBy <http://www.w3.org/2004/02/skos/core> ;
  rdfs:label "has exact match"@en ;
  rdfs:subPropertyOf skos:closeMatch ;
  skos:definition "skos:exactMatch is used to link two concepts, indicating a high degree of confidence that the concepts can be used interchangeably across a wide range of information retrieval applications. skos:exactMatch is a transitive property, and is a sub-property of skos:closeMatch."@en ;
.
skos:example
  a rdf:Property ;
  a owl:AnnotationProperty ;
  rdfs:isDefinedBy <http://www.w3.org/2004/02/skos/core> ;
  rdfs:label "example"@en ;
  rdfs:subPropertyOf skos:note ;
  skos:definition "An example of the use of a concept."@en ;
.
skos:hasTopConcept
  a rdf:Property ;
  a owl:ObjectProperty ;
  rdfs:domain skos:ConceptScheme ;
  rdfs:isDefinedBy <http://www.w3.org/2004/02/skos/core> ;
  rdfs:label "has top concept"@en ;
  rdfs:range skos:Concept ;
  owl:inverseOf skos:topConceptOf ;
  skos:definition "Relates, by convention, a concept scheme to a concept which is topmost in the broader/narrower concept hierarchies for that scheme, providing an entry point to these hierarchies."@en ;
.
skos:hiddenLabel
  a rdf:Property ;
  a owl:AnnotationProperty ;
  rdfs:comment "The range of skos:hiddenLabel is the class of RDF plain literals."@en ;
  rdfs:comment "skos:prefLabel, skos:altLabel and skos:hiddenLabel are pairwise disjoint properties."@en ;
  rdfs:isDefinedBy <http://www.w3.org/2004/02/skos/core> ;
  rdfs:label "hidden label"@en ;
  rdfs:subPropertyOf rdfs:label ;
  skos:definition "A lexical label for a resource that should be hidden when generating visual displays of the resource, but should still be accessible to free text search operations."@en ;
.
skos:historyNote
  a rdf:Property ;
  a owl:AnnotationProperty ;
  rdfs:isDefinedBy <http://www.w3.org/2004/02/skos/core> ;
  rdfs:label "history note"@en ;
  rdfs:subPropertyOf skos:note ;
  skos:definition "A note about the past state/use/meaning of a concept."@en ;
.
skos:inScheme
  a rdf:Property ;
  a owl:ObjectProperty ;
  rdfs:isDefinedBy <http://www.w3.org/2004/02/skos/core> ;
  rdfs:label "is in scheme"@en ;
  rdfs:range skos:ConceptScheme ;
  skos:definition "Relates a resource (for example a concept) to a concept scheme in which it is included."@en ;
  skos:scopeNote "A concept may be a member of more than one concept scheme."@en ;
.
skos:mappingRelation
  a rdf:Property ;
  a owl:ObjectProperty ;
  rdfs:comment "These concept mapping relations mirror semantic relations, and the data model defined below is similar (with the exception of skos:exactMatch) to the data model defined for semantic relations. A distinct vocabulary is provided for concept mapping relations, to provide a convenient way to differentiate links within a concept scheme from links between concept schemes. However, this pattern of usage is not a formal requirement of the SKOS data model, and relies on informal definitions of best practice."@en ;
  rdfs:isDefinedBy <http://www.w3.org/2004/02/skos/core> ;
  rdfs:label "is in mapping relation with"@en ;
  rdfs:subPropertyOf skos:semanticRelation ;
  skos:definition "Relates two concepts coming, by convention, from different schemes, and that have comparable meanings"@en ;
.
skos:member
  a rdf:Property ;
  a owl:ObjectProperty ;
  rdfs:domain skos:Collection ;
  rdfs:isDefinedBy <http://www.w3.org/2004/02/skos/core> ;
  rdfs:label "has member"@en ;
  rdfs:range [
      a owl:Class ;
      owl:unionOf (
          skos:Concept
          skos:Collection
        ) ;
    ] ;
  skos:definition "Relates a collection to one of its members."@en ;
.
skos:memberList
  a rdf:Property ;
  a owl:FunctionalProperty ;
  a owl:ObjectProperty ;
  rdfs:comment """For any resource, every item in the list given as the value of the
      skos:memberList property is also a value of the skos:member property."""@en ;
  rdfs:domain skos:OrderedCollection ;
  rdfs:isDefinedBy <http://www.w3.org/2004/02/skos/core> ;
  rdfs:label "has member list"@en ;
  rdfs:range rdf:List ;
  skos:definition "Relates an ordered collection to the RDF list containing its members."@en ;
.
skos:narrowMatch
  a rdf:Property ;
  a owl:ObjectProperty ;
  rdfs:isDefinedBy <http://www.w3.org/2004/02/skos/core> ;
  rdfs:label "has narrower match"@en ;
  rdfs:subPropertyOf skos:mappingRelation ;
  rdfs:subPropertyOf skos:narrower ;
  owl:inverseOf skos:broadMatch ;
  skos:definition "skos:narrowMatch is used to state a hierarchical mapping link between two conceptual resources in different concept schemes."@en ;
.
skos:narrower
  a rdf:Property ;
  a owl:ObjectProperty ;
  rdfs:comment "Narrower concepts are typically rendered as children in a concept hierarchy (tree)."@en ;
  rdfs:isDefinedBy <http://www.w3.org/2004/02/skos/core> ;
  rdfs:label "has narrower"@en ;
  rdfs:subPropertyOf skos:narrowerTransitive ;
  owl:inverseOf skos:broader ;
  skos:definition "Relates a concept to a concept that is more specific in meaning."@en ;
  skos:scopeNote "By convention, skos:broader is only used to assert an immediate (i.e. direct) hierarchical link between two conceptual resources."@en ;
.
skos:narrowerTransitive
  a rdf:Property ;
  a owl:ObjectProperty ;
  a owl:TransitiveProperty ;
  rdfs:isDefinedBy <http://www.w3.org/2004/02/skos/core> ;
  rdfs:label "has narrower transitive"@en ;
  rdfs:subPropertyOf skos:semanticRelation ;
  owl:inverseOf skos:broaderTransitive ;
  skos:definition "skos:narrowerTransitive is a transitive superproperty of skos:narrower." ;
  skos:scopeNote "By convention, skos:narrowerTransitive is not used to make assertions. Rather, the properties can be used to draw inferences about the transitive closure of the hierarchical relation, which is useful e.g. when implementing a simple query expansion algorithm in a search application."@en ;
.
skos:notation
  a rdf:Property ;
  a owl:DatatypeProperty ;
  rdfs:isDefinedBy <http://www.w3.org/2004/02/skos/core> ;
  rdfs:label "notation"@en ;
  skos:definition "A notation, also known as classification code, is a string of characters such as \"T58.5\" or \"303.4833\" used to uniquely identify a concept within the scope of a given concept scheme."@en ;
  skos:scopeNote "By convention, skos:notation is used with a typed literal in the object position of the triple."@en ;
.
skos:note
  a rdf:Property ;
  a owl:AnnotationProperty ;
  rdfs:isDefinedBy <http://www.w3.org/2004/02/skos/core> ;
  rdfs:label "note"@en ;
  skos:definition "A general note, for any purpose."@en ;
  skos:scopeNote "This property may be used directly, or as a super-property for more specific note types."@en ;
.
skos:prefLabel
  a rdf:Property ;
  a owl:AnnotationProperty ;
  rdfs:comment "A resource has no more than one value of skos:prefLabel per language tag."@en ;
  rdfs:comment "The range of skos:prefLabel is the class of RDF plain literals."@en ;
  rdfs:comment """skos:prefLabel, skos:altLabel and skos:hiddenLabel are pairwise
      disjoint properties."""@en ;
  rdfs:isDefinedBy <http://www.w3.org/2004/02/skos/core> ;
  rdfs:label "preferred label"@en ;
  rdfs:subPropertyOf rdfs:label ;
  skos:definition "The preferred lexical label for a resource, in a given language."@en ;
.
skos:related
  a rdf:Property ;
  a owl:ObjectProperty ;
  a owl:SymmetricProperty ;
  rdfs:comment "skos:related is disjoint with skos:broaderTransitive"@en ;
  rdfs:isDefinedBy <http://www.w3.org/2004/02/skos/core> ;
  rdfs:label "has related"@en ;
  rdfs:subPropertyOf skos:semanticRelation ;
  skos:definition "Relates a concept to a concept with which there is an associative semantic relationship."@en ;
.
skos:relatedMatch
  a rdf:Property ;
  a owl:ObjectProperty ;
  a owl:SymmetricProperty ;
  rdfs:isDefinedBy <http://www.w3.org/2004/02/skos/core> ;
  rdfs:label "has related match"@en ;
  rdfs:subPropertyOf skos:mappingRelation ;
  rdfs:subPropertyOf skos:related ;
  skos:definition "skos:relatedMatch is used to state an associative mapping link between two conceptual resources in different concept schemes."@en ;
.
skos:scopeNote
  a rdf:Property ;
  a owl:AnnotationProperty ;
  rdfs:isDefinedBy <http://www.w3.org/2004/02/skos/core> ;
  rdfs:label "scope note"@en ;
  rdfs:subPropertyOf skos:note ;
  skos:definition "A note that helps to clarify the meaning and/or the use of a concept."@en ;
.
skos:semanticRelation
  a rdf:Property ;
  a owl:ObjectProperty ;
  rdfs:domain skos:Concept ;
  rdfs:isDefinedBy <http://www.w3.org/2004/02/skos/core> ;
  rdfs:label "is in semantic relation with"@en ;
  rdfs:range skos:Concept ;
  skos:definition "Links a concept to a concept related by meaning."@en ;
  skos:scopeNote "This property should not be used directly, but as a super-property for all properties denoting a relationship of meaning between concepts."@en ;
.
skos:topConceptOf
  a rdf:Property ;
  a owl:ObjectProperty ;
  rdfs:domain skos:Concept ;
  rdfs:isDefinedBy <http://www.w3.org/2004/02/skos/core> ;
  rdfs:label "is top concept in scheme"@en ;
  rdfs:range skos:ConceptScheme ;
  rdfs:subPropertyOf skos:inScheme ;
  owl:inverseOf skos:hasTopConcept ;
  skos:definition "Relates a concept to the concept scheme that it is a top level concept of."@en ;
.
<https://linkeddata.cultureelerfgoed.nl/def/ztco>
  a owl:Ontology ;
  dcterms:created "2019-03-19" ;
  dcterms:creator ceo:Frans_van_der_Zande ;
  dcterms:creator ceo:Patrick_Mout ;
  dcterms:description "De ZTCO is de volledige semantische representatie van het logische datamodel Zaaktype uit de datalaag van de RCE"@nl ;
  dcterms:hasVersion "0.91" ;
  dcterms:license <https://creativecommons.org/licenses/by/4.0/> ;
  dcterms:publisher <http://standaarden.overheid.nl/owms/terms/Rijksdienst_voor_het_Cultureel_Erfgoed> ;
  dcterms:title "Zaak Type Catalogus Ontologie"@nl ;
  rdfs:label "Zaak Type Catalogus"@nl ;
  foaf:mbox "thesauri@cultureelerfgoed.nl" ;
.
ztco:AchisVeldwerkDatumafrondingRapport
  a ztco:Eigenschaptype ;
  rdfs:comment "De Eigenschaptype instantie ArchisVeldwerkDatumafrondingRapport wordt gebruikt om aan te geven welke Archis veldwerk datum afronding rapport is gekoppeld aan een zaak."@nl ;
  rdfs:label "Archis veldwerk: datum afronding rapport"@nl ;
  ztco:toelichtingEigenschaptype "Datum dat het archiseindonderzoeksrapport is ontvangen."@nl ;
.
ztco:Archis2Motief
  a ztco:Eigenschaptype ;
  dcterms:created "2019-03-27" ;
  dcterms:modified "" ;
  rdfs:comment "De Eigenschaptype instantie Archis2Motief wordt gebruikt om aan te geven welke Archis2 motief is gekoppeld aan een zaak."@nl ;
  rdfs:label "Archis2 motief"@nl ;
.
ztco:Archis2OnderzoeksId
  a ztco:Eigenschaptype ;
  dcterms:modified "2019-03-27" ;
  rdfs:comment "De Eigenschaptype instantie Archis2OnderzoeksId wordt gebruikt om aan te geven welke Archis2 onderzoeksidentificatie is gekoppeld aan een zaak."@nl ;
  rdfs:label "Archis2 onderzoeks_id"@nl ;
  ztco:toelichtingEigenschaptype "ID uit Archis2 tabel acs_onderzoeken"@nl ;
.
ztco:Archis2Onderzoeksmeldingsnummer
  a ztco:Eigenschaptype ;
  dcterms:modified "2019-03-27" ;
  rdfs:comment "De Eigenschaptype instantie Archis2Onderzoeksmeldingsnummer wordt gebruikt om aan te geven welke archis2onderzoeksmeldingsnummer is gekoppeld aan een zaak."@nl ;
  rdfs:label "Archis2onderzoeksmeldingsnummer"@nl ;
  ztco:toelichtingEigenschaptype "Archis2onderzoeksmeldingsnummer"@nl ;
.
ztco:Archis2Vondstmeldingsnummer
  a ztco:Eigenschaptype ;
  dcterms:modified "2019-03-27" ;
  rdfs:comment "De Eigenschaptype instantie Archis2Vondstmeldingsnummer wordt gebruikt om aan te geven welke Archis2 vondstmeldingsnummer is gekoppeld aan een zaak."@nl ;
  rdfs:label "Archis2 vondstmeldingsnummer"@nl ;
  ztco:toelichtingEigenschaptype "Mdg_id uit Archis2 tabel acs_waarnemingen"@nl ;
.
ztco:Archis2Waarnemingsnummer
  a ztco:Eigenschaptype ;
  dcterms:modified "2019-03-27" ;
  rdfs:comment "De Eigenschaptype instantie Archis2Waarnemingsnummer wordt gebruikt om aan te geven welke Archis2 waarnemingsnummer is gekoppeld aan een zaak."@nl ;
  rdfs:label "Archis2 waarnemingsnummer"@nl ;
  ztco:toelichtingEigenschaptype "Waarnemingsnummer uit Archis2 tabel acs_waarnemingen"@nl ;
.
ztco:ArchisVeldwerkBevoegdGezag
  a ztco:Eigenschaptype ;
  dcterms:modified "2019-03-27" ;
  rdfs:comment "De Eigenschaptype instantie ArchisVeldwerkBevoegdGezag wordt gebruikt om aan te geven welke Archis veldwerk bevoegd gezag is gekoppeld aan een zaak."@nl ;
  rdfs:label "Archis veldwerk: bevoegd gezag"@nl ;
  ztco:toelichtingEigenschaptype "Lijst van diversen betrokkenen als bevoegd gezag"@nl ;
  ztco:waardenverzamelingEigenschaptype "Gemeente;Waterschap;Provincie;Rijk;Geen" ;
.
ztco:ArchisVeldwerkDatumafronding
  a ztco:Eigenschaptype ;
  dcterms:modified "2019-03-27" ;
  rdfs:comment "De Eigenschaptype instantie ArchisVeldwerkDatumafronding wordt gebruikt om aan te geven welke Archis veldwerk datum afronding is gekoppeld aan een zaak."@nl ;
  rdfs:label "Archis veldwerk: datum afronding"@nl ;
  ztco:toelichtingEigenschaptype "Datum dat het archisonderzoek is afgerond."@nl ;
.
ztco:ArchisVeldwerkEinddatumGepland
  a ztco:Eigenschaptype ;
  dcterms:modified "2019-03-27" ;
  rdfs:comment "De Eigenschaptype instantie ArchisVeldwerkEinddatumGepland wordt gebruikt om aan te geven welke Archis veldwerk einddatum gepland is gekoppeld aan een zaak."@nl ;
  rdfs:label "Archis veldwerk: einddatum gepland"@nl ;
  ztco:toelichtingEigenschaptype "Veldwerk einddatum gepland"@nl ;
.
ztco:ArchisVeldwerkStartdatum
  a ztco:Eigenschaptype ;
  dcterms:modified "2019-03-27" ;
  rdfs:comment "De Eigenschaptype instantie ArchisVeldwerkStartdatum wordt gebruikt om aan te geven welke Archis veldwerk startdatum is gekoppeld aan een zaak."@nl ;
  rdfs:label "Archis veldwerk: startdatum"@nl ;
  ztco:toelichtingEigenschaptype "Veldwerk startdatum"@nl ;
.
ztco:ArchisVeldwerkVerwachteDatumAfrondingRapport
  a ztco:Eigenschaptype ;
  dcterms:modified "2019-03-27" ;
  rdfs:comment "De Eigenschaptype instantie AchisVeldwerkVerwachteDatumAfrondingRapport wordt gebruikt om aan te geven welke Archis veldwerk verwachte datum afronding rapport is gekoppeld aan een zaak."@nl ;
  rdfs:label "Archis veldwerk: verwachte datum afronding rapport"@nl ;
  ztco:toelichtingEigenschaptype "Veldwerk verwachte datum afronding rapport"@nl ;
.
ztco:ArchisVondstmeldingDatumVondst
  a ztco:Eigenschaptype ;
  dcterms:modified "2019-03-27" ;
  rdfs:comment "De Eigenschaptype instantie ArchisVondstmeldingDatumVondst wordt gebruikt om aan te geven welke Archis vondstmelding datum vondst is gekoppeld aan een zaak."@nl ;
  rdfs:label "Archis Vondstmelding Datum Vondst"@nl ;
  ztco:toelichtingEigenschaptype "Datum van vondstmelding."@nl ;
.
ztco:Besluittype
  a owl:Class ;
  rdfs:comment "De class ztco:Besluittype is een representatie van de generieke aanduiding van de aard van een besluit."@nl ;
  rdfs:label "Besluittype"@nl ;
  rdfs:subClassOf owl:Thing ;
  skos:definition "Generieke aanduiding van de aard van een besluit"@nl ;
.
ztco:Documenttype
  a owl:Class ;
  rdfs:comment "De class ztco:Documenttype is een representatie van de aanduiding van de aard van een document zoals gehanteerd door RCE."@nl ;
  rdfs:label "Documenttype"@nl ;
  rdfs:subClassOf owl:Thing ;
  skos:definition "Aanduiding van de aard van een document zoals gehanteerd door RCE."@nl ;
.
ztco:Eigenschaptype
  a owl:Class ;
  rdfs:comment "De class ztco:Eigenschaptype is een representatie van een relevant inhoudelijk gegeven dat bij zaken van dit zaaktype geregistreerd moet kunnen worden en geen standaard kenmerk is van een zaaktype."@nl ;
  rdfs:label "Eigenschaptype"@nl ;
  rdfs:subClassOf owl:Thing ;
  skos:definition "Een relevant inhoudelijk gegeven dat bij zaken van dit zaaktype geregistreerd moet kunnen worden en geen standaard kenmerk is van een zaaktype."@nl ;
.
ztco:MRSprojectcode
  a ztco:Eigenschaptype ;
  dcterms:modified "2019-03-27" ;
  rdfs:comment "De Eigenschaptype instantie MRSprojectcode wordt gebruikt om aan te geven welke  MRS projectcode is gekoppeld aan een zaak."@nl ;
  rdfs:label "Mrsprojectcode"@nl ;
  ztco:toelichtingEigenschaptype "De verschillende MRS-Projecten binnen RCE"@nl ;
  ztco:waardenverzamelingEigenschaptype "Wederopbouw 1940-1958 ;Nieuwe Hollandse Waterlinie ;MSP ;Archeologie 2008 ;Archeologie 2013 ;Wederopbouw 1959-1965 ;WKPB ;Vestingwerken ;Verbetervoorstellen algemeen ;Verbetervoorstellen Molens ;Verbetervoorstellen Kerken ;Verbetervoorstellen Utrecht bruggen ;Verbetervoorstellen subsidies " ;
.
ztco:Roltype
  a owl:Class ;
  rdfs:comment "De class ztco:Roltype is een representatie van de generieke aanduiding van de aard van een rol die een betrokkene kan uitoefenen in zaken van een zaaktype."@nl ;
  rdfs:label "Roltype"@nl ;
  rdfs:subClassOf owl:Thing ;
  skos:definition "Generieke aanduiding van de aard van een ROL die een betrokkene kan uitoefenen in zaken van een zaaktype."@nl ;
.
ztco:Statustype
  a owl:Class ;
  rdfs:comment "De class ztco:Statustype is een representatie van de generieke aanduiding van de aard van een status."@nl ;
  rdfs:label "Statustype"@nl ;
  rdfs:subClassOf owl:Thing ;
  skos:definition "Generieke aanduiding van de aard van een status."@nl ;
.
ztco:Zaaktype
  a owl:Class ;
  rdfs:comment "De class ztco:Zaaktype is een representatie van de generieke aanduiding van de aard van een zaak."@nl ;
  rdfs:label "zaaktype"@nl ;
  rdfs:subClassOf owl:Thing ;
  skos:definition "Generieke aanduiding van de aard van een zaak."@nl ;
.
ztco:aanleiding
  a owl:DatatypeProperty ;
  rdfs:comment "De property aanleiding wordt gebruikt om aan te geven welke aanleiding is gekoppeld aan een zaaktype."@nl ;
  rdfs:domain ztco:Zaaktype ;
  rdfs:label "Aanleiding"@nl ;
  rdfs:range xsd:string ;
  skos:definition "Een omschrijving van de gebeurtenis/trigger die leidt tot het starten van een zaak van dit zaaktype. Dit veld heeft vooral een documentatiefunctie en is bedoeld om een omschrijving te geven van de gebeurtenis - de gedefinieerde aanleiding uit de definitie van een zaak - die leidt tot zaaken van dit zaaktype. Denk bij het uitwerken ook aan de kanalen waarlangs deze trigger kan binnenkomen. "@nl ;
.
ztco:archiefnominatie
  a owl:DatatypeProperty ;
  rdfs:comment "De property archiefnominatie wordt gebruikt om aan te geven welke archiefnominatie is gekoppeld aan een zaaktype."@nl ;
  rdfs:domain ztco:Zaaktype ;
  rdfs:label "Archiefnominatie"@nl ;
  rdfs:range xsd:string ;
  skos:definition "Aanduiding die aangeeft of zaken van dit zaaktype blijvend moeten worden bewaard, vernietigd of overgebracht naar een archiefbewaarplaats. Bij vernietiging en overbrenging wordt middels het veld Archieftermijn aangegeven na verloop van hoeveel tijd wordt overgegaan tot vernietiging c.q. overbrenging. De waarde 'O' voor overbrenging dient uitsluitend te worden gebruikt indien - conform art. 13 van de Archiefwet 1995 - eerder of later dan na verloop van de in art. 12 van de Archiefwet 1995 bepaalde algemene termijn van 20 jaar wordt overgegaan tot overbrenging. Waardenverzameling: B: Blijvend bewaren, V: Vernietigen, O: Overbrengen (van blijvend te bewaren archiefbescheiden)."@nl ;
.
ztco:archieftermijn
  a owl:DatatypeProperty ;
  rdfs:comment "De property archieftermijn wordt gebruikt om aan te geven welke archieftermijn is gekoppeld aan een zaaktype."@nl ;
  rdfs:domain ztco:Zaaktype ;
  rdfs:label "Archieftermijn"@nl ;
  rdfs:range xsd:integer ;
  skos:definition "De termijn in maanden waarna het zaakdossier (de zaak met alle bijbehorende documenten) van een zaak van dit type vernietigd of overgebracht moet worden."@nl ;
.
ztco:besluittypeOmschrijving
  a owl:DatatypeProperty ;
  dcterms:modified "2019-03-20" ;
  rdfs:comment "De property besluittypeOmschrijving wordt gebruikt om aan te geven welke omschrijving is gekoppeld aan een besluittype."@nl ;
  rdfs:domain ztco:Besluittype ;
  rdfs:label "Besluittypeomschrijving"@nl ;
  rdfs:range xsd:string ;
  skos:definition "Omschrijving van de aard van besluiten van het besluitype."@nl ;
.
ztco:brondatumArchiefprocedure
  a owl:DatatypeProperty ;
  rdfs:comment "De property brondatumArchiefprocedure wordt gebruikt om aan te geven welke brondatum archiefprocedure is gekoppeld aan een zaaktype."@nl ;
  rdfs:domain ztco:Zaaktype ;
  rdfs:label "Brondatum archiefprocedure"@nl ;
  rdfs:range xsd:date ;
  skos:definition "Welk datumveld geldt als de start van de bewaar- of overbrengingstermijn, per zaaktype kan een andere soort datum gelden als brondatum."@nl ;
.
ztco:datumBeginGeldigheidBesluittype
  a owl:DatatypeProperty ;
  rdfs:comment "De property datumBeginGeldigheidBesluittype wordt gebruikt om aan te geven welke begindatum geldigheid is gekoppeld aan een besluittype."@nl ;
  rdfs:domain ztco:Besluittype ;
  rdfs:label "Datum begin geldigheid besluittype"@nl ;
  rdfs:range xsd:date ;
  skos:definition "De datum van wanneer het besluittype geldig is."@nl ;
.
ztco:datumBeginGeldigheidDocumenttype
  a owl:DatatypeProperty ;
  dcterms:modified "2019-03-20" ;
  rdfs:comment "De property datumBeginGeldigheiddocumenttype wordt gebruikt om aan te geven welke begindatum geldigheid is gekoppeld aan een documenttype."@nl ;
  rdfs:domain ztco:Documenttype ;
  rdfs:label "Datum begin geldigheid documenttype"@nl ;
  rdfs:range xsd:date ;
  skos:definition "De datum van wanneer het documenttype geldig is."@nl ;
.
ztco:datumBeginGeldigheidStatustype
  a owl:DatatypeProperty ;
  dcterms:modified "2019-03-20" ;
  rdfs:comment "De property datumBeginGeldigheidStatustype wordt gebruikt om aan te geven welke begindatum geldigheid is gekoppeld aan een statustype."@nl ;
  rdfs:domain ztco:Statustype ;
  rdfs:label "Datum begin geldigheid statustype"@nl ;
  rdfs:range xsd:date ;
  skos:definition "De begindatum waarop het statustype is geldig is."@nl ;
.
ztco:datumBeginGeldigheidZaaktype
  a owl:DatatypeProperty ;
  dcterms:modified "2019-03-20" ;
  rdfs:comment "De property datumBeginGeldigheidZaaktype wordt gebruikt om aan te geven welke begindatum geldigheid is gekoppeld aan een zaaktype."@nl ;
  rdfs:domain ztco:Zaaktype ;
  rdfs:label "Datum begin geldigheid zaaktype"@nl ;
  rdfs:range xsd:date ;
  skos:definition "De datum van wanneer het zaaktype geldig is."@nl ;
.
ztco:datumEindeGeldigheidBesluittype
  a owl:DatatypeProperty ;
  rdfs:comment "De property datumEindeGeldigheidBesluittype wordt gebruikt om aan te geven welke einddatum geldigheid is gekoppeld aan een besluittype."@nl ;
  rdfs:domain ztco:Besluittype ;
  rdfs:label "Datum einde geldigheid besluittype"@nl ;
  rdfs:range xsd:date ;
  skos:definition "De datum van wanneer het besluittype niet meer geldig is."@nl ;
.
ztco:datumEindeGeldigheidDocumenttype
  a owl:DatatypeProperty ;
  dcterms:modified "2019-03-20" ;
  rdfs:comment "De property datumEindeGeldigheiddocumenttype wordt gebruikt om aan te geven welke einddatum geldigheid is gekoppeld aan een documenttype."@nl ;
  rdfs:domain ztco:Documenttype ;
  rdfs:label "Datum einde geldigheid documenttype"@nl ;
  rdfs:range xsd:date ;
  skos:definition "De datum van wanneer het documenttype niet meer geldig is."@nl ;
.
ztco:datumEindeGeldigheidStatustype
  a owl:DatatypeProperty ;
  dcterms:modified "20129-03-20" ;
  rdfs:comment "De property datumEindeGeldigheidStatustype wordt gebruikt om aan te geven welke datum einde geldigheid is gekoppeld aan een statustype."@nl ;
  rdfs:domain ztco:Statustype ;
  rdfs:label "Datum einde geldigheid statustype"@nl ;
  rdfs:range xsd:date ;
  skos:definition "De datum waarop het statustype niet meer geldig is."@nl ;
.
ztco:datumEindeGeldigheidZaaktype
  a owl:DatatypeProperty ;
  dcterms:modified "2019-03-20" ;
  rdfs:comment "De property datumEindeGeldigheidZaaktype wordt gebruikt om aan te geven welke einddatumdatum geldigheid  is gekoppeld aan een zaaktype."@nl ;
  rdfs:domain ztco:Zaaktype ;
  rdfs:label "Datum einde geldigheid zaaktype"@nl ;
  rdfs:range xsd:date ;
  skos:definition "De datum van wanneer het zaaktype niet meer geldig is."@nl ;
.
ztco:datumUitstelRapportverplichting
  a ztco:Eigenschaptype ;
  dcterms:modified "2019-03-27" ;
  rdfs:comment "De Eigenschaptype instantie datumUitstelRapportverplichting wordt gebruikt om aan te geven welke datum uitstel rapportverplichting is gekoppeld aan een zaak."@nl ;
  rdfs:label "Datum uitstel rapportverplichting"@nl ;
  ztco:toelichtingEigenschaptype "Datum uitstel rapportverplichting"@nl ;
.
ztco:definitieEigenschaptype
  a owl:DatatypeProperty ;
  dcterms:modified "2019-03-04" ;
  rdfs:comment "De property definitieEigenschaptype wordt gebruikt om aan te geven welke definitie is gekoppeld aan een eigenschaptype."@nl ;
  rdfs:domain ztco:Eigenschaptype ;
  rdfs:label "Definitie eigenschaptype"@nl ;
  rdfs:range xsd:string ;
  skos:definition "De beschrijving van de betekenis van deze eigenschap"@nl ;
.
ztco:documenttypeOmschrijving
  a owl:DatatypeProperty ;
  dcterms:modified "2019-03-20" ;
  rdfs:comment "De property documenttypeOmschrijving wordt gebruikt om aan te geven welke omschrijving is gekoppeld aan een documenttype."@nl ;
  rdfs:domain ztco:Documenttype ;
  rdfs:label "Documenttype omschrijving"@nl ;
  rdfs:range xsd:string ;
  skos:definition "Omschrijving van de aard van documenten van dit documenttype."@nl ;
.
ztco:doel
  a owl:DatatypeProperty ;
  rdfs:comment "De property doel wordt gebruikt om aan te geven welke doel is gekoppeld aan een zaaktype."@nl ;
  rdfs:domain ztco:Zaaktype ;
  rdfs:label "Doel "@nl ;
  rdfs:range xsd:string ;
  skos:definition "Een omschrijving van wat het doel is. Dit veld heeft vooral een documentatiefunctie en is bedoeld om een omschrijving te geven van het doel dat wordt nagestreefd in zaaken van dit zaaktype. Denk aan het beoordelen van een subsidie aanvraag met het oogmerk daarover een besluit te nemen, het innemen van een standpunt na aanleiding van een ingediend bezwaar, et cetera. "@nl ;
.
ztco:doorlooptijdBehandeling
  a owl:DatatypeProperty ;
  dcterms:modified "2019-02-20" ;
  rdfs:comment "De property doorlooptijdBehandeling wordt gebruikt om aan te geven welke doorlooptijd behandeling is gekoppeld aan een zaaktype."@nl ;
  rdfs:domain ztco:Zaaktype ;
  rdfs:label "Doorlooptijd behandeling"@nl ;
  rdfs:range xsd:string ;
  skos:definition "De periode waarbinnen volgens wet- en regelgeving een zaak van het zaaktype afgerond dient te zijn"@nl ;
.
ztco:doorlooptijdStatus
  a owl:DatatypeProperty ;
  rdfs:comment "De property doorlooptijdStatus wordt gebruikt om aan te geven welke doorlooptijd status is gekoppeld aan een statustype."@nl ;
  rdfs:domain ztco:Statustype ;
  rdfs:label "Doorlooptijd status"@nl ;
  rdfs:range xsd:integer ;
  skos:definition "De door de RCE gestelde norm voor de doorlooptijd voor het bereiken van statussen van dit statustype bij het desbetreffende zaaktype."@nl ;
.
ztco:eerdereZaken
  a ztco:Eigenschaptype ;
  dcterms:modified "2019-03-27" ;
  rdfs:comment "De Eigenschaptype instantie eerdereZaken wordt gebruikt om aan te geven welke eerdere zaken zijn gekoppeld aan een zaak."@nl ;
  rdfs:label "Eerdere zaken"@nl ;
  ztco:toelichtingEigenschaptype "Geeft aan welke andere zaken betrekking hebben op dit onderzoek/zaak"@nl ;
.
ztco:eigenschapnaamEigenschaptype
  a owl:DatatypeProperty ;
  dcterms:modified "2019-03-04" ;
  rdfs:comment "De property eigenschapnaamEigenschaptype wordt gebruikt om aan te geven welke eigenschapnaam is gekoppeld aan een eigenschaptype."@nl ;
  rdfs:domain ztco:Eigenschaptype ;
  rdfs:label "Eigenschapnaam eigenschaptype"@nl ;
  rdfs:range xsd:string ;
  skos:definition "De naam van de eigenschap"@nl ;
.
ztco:formaatEigenschaptype
  a owl:DatatypeProperty ;
  dcterms:modified "2019-03-04" ;
  rdfs:comment "De property formaatEigenschaptype wordt gebruikt om aan te geven welke formaat is gekoppeld aan een eigenschaptype."@nl ;
  rdfs:domain ztco:Eigenschaptype ;
  rdfs:label "Formaat eigenschaptype"@nl ;
  rdfs:range xsd:string ;
  skos:definition "Het soort tekens waarmee waarden van de eigenschap kunnen worden vastgelegd."@nl ;
.
ztco:formuliernaam
  a owl:DatatypeProperty ;
  rdfs:comment "De property formuliernaam wordt gebruikt om aan te geven welke formuliernaam is gekoppeld aan een zaaktype."@nl ;
  rdfs:domain ztco:Zaaktype ;
  rdfs:label "Formuliernaam"@nl ;
  rdfs:range xsd:string ;
  skos:definition "De naam van het formulier, waarmee de klant het product of dienst kan aanvragen. "@nl ;
.
ztco:heeftBetrekkingOpAndereZaaktype
  a owl:SymmetricProperty ;
  dcterms:created "2019-03-12" ;
  dcterms:modified "" ;
  rdfs:comment "De property heeftBetrekkingOpAndereZaaktype legt de relatie tussen zaaktype en zaaktype vast."@nl ;
  rdfs:domain ztco:Zaaktype ;
  rdfs:label "heeft betrekking op andere zaaktype" ;
  rdfs:range ztco:Zaaktype ;
.
ztco:heeftBetrekkingOpZaaktype
  a owl:ObjectProperty ;
  dcterms:modified "2019-03-12" ;
  rdfs:comment "De property heeftBetrekkingOpZaaktype legt de relatie tussen statustype en zaaktype vast."@nl ;
  rdfs:domain ztco:Statustype ;
  rdfs:label "Heeft betrekking op zaaktype"@nl ;
  rdfs:range ztco:Zaaktype ;
  owl:inverseOf ztco:heeftStatustype ;
.
ztco:heeftBetrokkeneInRoltype
  a owl:ObjectProperty ;
  dcterms:modified "2019-02-20" ;
  rdfs:comment "De property heeftBetrokkeneInRoltype legt de relatie tussen zaaktype en roltype vast."@nl ;
  rdfs:domain ztco:Zaaktype ;
  rdfs:label "Heeft betrokkene in roltype"@nl ;
  rdfs:range ztco:Roltype ;
  owl:inverseOf ztco:heeftBetrokkeneOpZaaktype ;
  skos:definition "Het zaaktype van zaken waarin betrokkenen rollen van dit roltype kunnen uitoefenen."@nl ;
.
ztco:heeftBetrokkeneOpZaaktype
  a owl:ObjectProperty ;
  dcterms:created "2019-02-20" ;
  dcterms:modified "" ;
  rdfs:comment "De property heeftBetrokkeneOpZaaktype legt de relatie tussen roltype en zaaktype vast."@nl ;
  rdfs:domain ztco:Roltype ;
  rdfs:label "Heeft betrokkene op zaaktype"@nl ;
  rdfs:range ztco:Zaaktype ;
  owl:inverseOf ztco:heeftBetrokkeneInRoltype ;
.
ztco:heeftDeelzakenZaaktype
  a owl:ObjectProperty ;
  dcterms:modified "2019-02-20" ;
  rdfs:comment "De property heeftDeelzakenZaaktype legt de relatie tussen deelzaken en zaaktype vast."@nl ;
  rdfs:domain ztco:Zaaktype ;
  rdfs:label "Heeft deelzaken zaaktype"@nl ;
  rdfs:range ztco:Zaaktype ;
  owl:inverseOf ztco:isDeelzakenVanZaaktype ;
.
ztco:heeftEigenschaptype
  a owl:ObjectProperty ;
  dcterms:created "2019-02-20" ;
  dcterms:modified "" ;
  rdfs:comment "De property heeftEigenschaptype legt de relatie tussen zaaktype en eigenschaptype vast."@nl ;
  rdfs:domain ztco:Zaaktype ;
  rdfs:label "heeft eigenschaptype"@nl ;
  rdfs:range ztco:Eigenschaptype ;
.
ztco:heeftEigenschapwaardeNaam
  a owl:ObjectProperty ;
  dcterms:created "" ;
  dcterms:modified "2019-03-20" ;
  rdfs:comment "De property heeftEigenschapwaardeNaam legt de relatie tussen eigenschaptype en waarde vast."@nl ;
  rdfs:domain ztco:Eigenschaptype ;
  rdfs:label "heeft eigenschapwaarde naam" ;
  rdfs:range skos:Concept ;
.
ztco:heeftRelevanteDocumentype
  a owl:ObjectProperty ;
  dcterms:modified "2019-02-20" ;
  rdfs:comment "De property heeftRelevanteDocumenttype legt de relatie tussen zaaktype en documenttype vast."@nl ;
  rdfs:domain ztco:Zaaktype ;
  rdfs:label "Heeft relevante documenttype"@nl ;
  rdfs:range ztco:Documenttype ;
  owl:inverseOf ztco:isRelevantVoorZaaktype ;
  skos:definition "De documenttypen die relevant kunnen zijn voor zaken van dit zaaktype."@nl ;
.
ztco:heeftStatustype
  a owl:ObjectProperty ;
  dcterms:modified "2019-03-12" ;
  rdfs:comment "De property heeftStatustype legt de relatie tussen zaaktype en statustype vast."@nl ;
  rdfs:domain ztco:Zaaktype ;
  rdfs:label "Heeft statustype"@nl ;
  rdfs:range ztco:Statustype ;
  owl:inverseOf ztco:heeftBetrekkingOpZaaktype ;
  skos:definition "De statustypen die bereikt kunnen worden bij behandeling van zaken van het zaaktype."@nl ;
.
ztco:hoortBijDocumenttype
  a owl:ObjectProperty ;
  dcterms:created "2019-02-20" ;
  dcterms:modified "" ;
  rdfs:comment "De property hoortBijDocumenttype legt de relatie tussen statustype en documenttype vast."@nl ;
  rdfs:domain ztco:Statustype ;
  rdfs:label "Hoort bij documenttype"@nl ;
  rdfs:range ztco:Documenttype ;
  owl:inverseOf ztco:verplichtBijStatustype ;
.
ztco:isDeelzakenVanZaaktype
  a owl:ObjectProperty ;
  dcterms:created "2019-02-20" ;
  dcterms:modified "" ;
  rdfs:comment "De property isDeelzakenVanZaaktype legt de relatie tussen zaaktype en deelzaken vast."@nl ;
  rdfs:domain ztco:Zaaktype ;
  rdfs:label "Is deelzaken van zaaktype"@nl ;
  rdfs:range ztco:Zaaktype ;
  owl:inverseOf ztco:heeftDeelzakenZaaktype ;
.
ztco:isGezetDoorRoltype
  a owl:ObjectProperty ;
  dcterms:created "2019-02-20" ;
  dcterms:modified "" ;
  rdfs:comment "De property isGezetDoorRoltype legt de relatie tussen statustype en roltype vast."@nl ;
  rdfs:domain ztco:Statustype ;
  rdfs:label "is gezet door roltype"@nl ;
  rdfs:range ztco:Roltype ;
  owl:inverseOf ztco:zetAlsBetrokkeneStatustype ;
.
ztco:isRelevantVoorZaaktype
  a owl:ObjectProperty ;
  dcterms:created "2019-02-20" ;
  dcterms:modified "" ;
  rdfs:comment "De property IsRelevantVoorZaaktype legt de relatie tussen documenttype en zaakttype vast."@nl ;
  rdfs:domain ztco:Documentype ;
  rdfs:label "is relevant voor zaaktype"@nl ;
  rdfs:range ztco:Zaaktype ;
  owl:inverseOf ztco:heeftRelevanteDocumentype ;
.
ztco:kardinaliteitEigenschaptype
  a owl:DatatypeProperty ;
  dcterms:modified "2019-03-04" ;
  rdfs:comment "De property kardinaliteitEigenschaptype wordt gebruikt om aan te geven welke kardinaliteit is gekoppeld aan een eigenschaptype."@nl ;
  rdfs:domain ztco:Eigenschaptype ;
  rdfs:label "Kardinaliteit eigenschaptype"@nl ;
  rdfs:range xsd:integer ;
  skos:definition "Het aantal mogelijke voorkomens van deze eigenschap binnen het zaaktype."@nl ;
.
ztco:legtVastBesluit
  a owl:ObjectProperty ;
  dcterms:created "2019-02-20" ;
  dcterms:modified "" ;
  rdfs:comment "De property legtVastBesluit legt de relatie tussen documenttype en besluittype vast."@nl ;
  rdfs:domain ztco:Documentype ;
  rdfs:label "Legt vast besluit"@nl ;
  rdfs:range ztco:Besluitype ;
  owl:inverseOf ztco:wordtVastgelegdInDocumenttype ;
.
ztco:lengteEigenschaptype
  a owl:DatatypeProperty ;
  dcterms:modified "2019-03-04" ;
  rdfs:comment "De property lengteEigenschaptype wordt gebruikt om aan te geven welke lengte is gekoppeld aan een eigenschaptype."@nl ;
  rdfs:domain ztco:Eigenschaptype ;
  rdfs:label "Lengte eigenschaptype"@nl ;
  rdfs:range xsd:integer ;
  skos:definition "Het aantal karakters (lengte) waarmee waarden van de eigenschap worden vastgelegd."@nl ;
.
ztco:onderzoeksnaam
  a ztco:Eigenschaptype ;
  dcterms:modified "2019-03-27" ;
  rdfs:comment "De Eigenschaptype instantie onderzoeksnaam wordt gebruikt om aan te geven welke onderzoeksnaam is gekoppeld aan een zaak."@nl ;
  rdfs:label "Onderzoeksnaam"@nl ;
  ztco:toelichtingEigenschaptype "Naam die de onderzoeker aan het onderzoek heeft gegeven."@nl ;
.
ztco:opdrachtstype
  a ztco:Eigenschaptype ;
  dcterms:created "2019-03-27" ;
  dcterms:modified "" ;
  rdfs:comment "De Eigenschaptype instantie opdrachtstype wordt gebruikt om aan te geven welk opdrachtstype is gekoppeld aan een zaak."@nl ;
  rdfs:label "opdrachtstype" ;
  ztco:waardenverzamelingEigenschaptype "WKPB" ;
.
ztco:perceel
  a ztco:Eigenschaptype ;
  dcterms:created "2019-03-27" ;
  dcterms:modified "" ;
  rdfs:comment "De Eigenschaptype instantie perceel wordt gebruikt om aan te geven welk perceel is gekoppeld aan een zaak."@nl ;
  rdfs:label "Perceel"@nl ;
.
ztco:procesnaam
  a owl:DatatypeProperty ;
  rdfs:comment "De property procesnaam wordt gebruikt om aan te geven welke procesnaam is gekoppeld aan een zaaktype."@nl ;
  rdfs:domain ztco:Zaaktype ;
  rdfs:label "Procesnaam"@nl ;
  rdfs:range xsd:string ;
  skos:definition "Naam van het proces dat het zaaktype uitvoert."@nl ;
.
ztco:productDienst
  a owl:DatatypeProperty ;
  rdfs:comment "De property productDienst wordt gebruikt om aan te geven welke product/dienst is gekoppeld aan een zaaktype."@nl ;
  rdfs:domain ztco:Zaaktype ;
  rdfs:label "Product/Dienst"@nl ;
  rdfs:range xsd:string ;
  skos:definition "Het product of de dienst die geleverd wordt door dit zaaktype. "@nl ;
.
ztco:reactietermijn
  a owl:DatatypeProperty ;
  rdfs:comment "De property reactietermijn wordt gebruikt om aan te geven welke reactietermijn is gekoppeld aan een besluittype."@nl ;
  rdfs:domain ztco:Besluittype ;
  rdfs:label "Reactietermijn"@nl ;
  rdfs:range xsd:integer ;
  skos:definition "Het aantal dagen, gerekend vanaf de verzend- of publicatiedatum, waarbinnen verweer tegen een besluit van het besluittype mogelijk is."@nl ;
.
ztco:regime
  a ztco:Eigenschaptype ;
  dcterms:modified "2019-03-27" ;
  rdfs:comment "De Eigenschaptype instantie regime wordt gebruikt om aan te geven welke regime is gekoppeld aan een zaak."@nl ;
  rdfs:label "Regime"@nl ;
  ztco:toelichtingEigenschaptype "Onder welk regime heeft de zaak plaats"@nl ;
  ztco:waardenverzamelingEigenschaptype "Monumentenwet1988;Erfgoedwet2016" ;
.
ztco:reikwijdte
  a ztco:Eigenschaptype ;
  dcterms:modified "2019-03-27" ;
  rdfs:comment "De Eigenschaptype instantie reikwijdte wordt gebruikt om aan te geven welke reikwijdte is gekoppeld aan een zaak."@nl ;
  rdfs:label "Reikwijdte"@nl ;
  ztco:toelichtingEigenschaptype "reikwijdte van de zaak"@nl ;
  ztco:waardenverzamelingEigenschaptype "Kort;Lang;Administratief" ;
.
ztco:restauratieHypotheekBedrag
  a ztco:Eigenschaptype ;
  dcterms:created "2019-03-27" ;
  dcterms:modified "" ;
  rdfs:comment "De Eigenschaptype instantie restauratieHypotheekBedragwordt gebruikt om aan te geven welk restauratie hypotheek bedrag is gekoppeld aan een zaak."@nl ;
  rdfs:label "Restauratie hypotheek bedrag"@nl ;
.
ztco:roltypeomschrijving
  a owl:DatatypeProperty ;
  dcterms:modified "2019-03-20" ;
  rdfs:comment "De property roltypeomschrijving wordt gebruikt om aan te geven welke omschrijving is gekoppeld aan een roltype."@nl ;
  rdfs:domain ztco:Roltype ;
  rdfs:label "Roltypeomschrijving"@nl ;
  rdfs:range xsd:string ;
  skos:definition "Omschrijving van de aard van de rol."@nl ;
.
ztco:selectielijstTekst
  a owl:DatatypeProperty ;
  rdfs:comment "De property selectielijstTekst wordt gebruikt om aan te geven welke selectielijst tekst is gekoppeld aan een zaaktype."@nl ;
  rdfs:domain ztco:Zaaktype ;
  rdfs:label "Selectielijst tekst"@nl ;
  rdfs:range xsd:string ;
  skos:definition "De relevante tekst die voor dit zaaktype dient te worden / is opgenomen in het Basisselectiedocument betreffende de eisen vanuit archivering."@nl ;
.
ztco:servicenormBehandeling
  a owl:DatatypeProperty ;
  rdfs:comment "De property servicenormBehandeling wordt gebruikt om aan te geven welke servicenorm behandeling is gekoppeld aan een zaaktype."@nl ;
  rdfs:domain ztco:Zaaktype ;
  rdfs:label "Servicenorm behandeling"@nl ;
  rdfs:range xsd:string ;
  skos:definition "De periode waarbinnen verwacht wordt dat een zaak van het zaaktype afgerond wordt conform de geldende servicenormen van RCE"@nl ;
.
ztco:soortBetrokkene
  a owl:DatatypeProperty ;
  rdfs:comment "De property soortBetrokkene wordt gebruikt om aan te geven welke soort betrokkene is gekoppeld aan een roltype."@nl ;
  rdfs:domain ztco:Roltype ;
  rdfs:label "Soort betrokkene"@nl ;
  rdfs:range xsd:string ;
  skos:definition "De (soort) betrokkene die een rol van dit roltype mag uitoefenen."@nl ;
.
ztco:statustypeOmschrijving
  a owl:DatatypeProperty ;
  dcterms:modified "2019-03-20" ;
  rdfs:comment "De property statustypeOmschrijving wordt gebruikt om aan te geven welke omschrijving is gekoppeld aan een statustype."@nl ;
  rdfs:domain ztco:Statustype ;
  rdfs:label "Statustypeomschrijving"@nl ;
  rdfs:range xsd:string ;
  skos:definition "Een korte, voor de initiator van de zaak relevante, omschrijving van de aard van de status van zaken van een zaaktype."@nl ;
.
ztco:statustypevolgnummer
  a owl:DatatypeProperty ;
  dcterms:modified "2019-03-20" ;
  rdfs:comment "De property statustypevolgnummer wordt gebruikt om aan te geven welk volgnummer is gekoppeld aan een statustype."@nl ;
  rdfs:domain ztco:Statustype ;
  rdfs:label "Statustypevolgnummer"@nl ;
  rdfs:range xsd:integer ;
  skos:definition "Een volgnummer voor de status binnen een zaak."@nl ;
.
ztco:toelichtingBesluittype
  a owl:DatatypeProperty ;
  rdfs:comment "De property toelichtingBesluittype wordt gebruikt om aan te geven welke toelichting is gekoppeld aan een besluittype."@nl ;
  rdfs:domain ztco:Besluittype ;
  rdfs:label "Toelichting besluittype"@nl ;
  rdfs:range xsd:string ;
  skos:definition "Een eventuele toelichting op dit besluittype. Dit veld heeft vooral een documentatiefunctie en is bedoeld om een toelichting te geven op dit besluittype. Hier kan bijvoorbeeld een beschrijving worden gegeven van de betekenis van het besluit voor - het verloop van - een zaaktype."@nl ;
.
ztco:toelichtingDocumenttype
  a owl:DatatypeProperty ;
  rdfs:comment "De property toelichtingDocumenttype wordt gebruikt om aan te geven welke toelichting is gekoppeld aan een documenttype."@nl ;
  rdfs:domain ztco:Documenttype ;
  rdfs:label "Toelichting documenttype"@nl ;
  rdfs:range xsd:string ;
  skos:definition "Een eventuele toelichting op dit documenttype. Dit veld heeft vooral een documentatiefunctie en is bedoeld om een toelichting te geven op dit documenttype. Hier kan bijvoorbeeld een beschrijving worden gegeven van de betekenis van het documenttype en de aard van de documenten die ertoe behoren."@nl ;
.
ztco:toelichtingEigenschaptype
  a owl:DatatypeProperty ;
  rdfs:comment "De property toelichtingEigenschaptype wordt gebruikt om aan te geven welke toelichting is gekoppeld aan een Eigenschaptype."@nl ;
  rdfs:domain ztco:Eigenschaptype ;
  rdfs:label "Toelichting eigenschaptype"@nl ;
  rdfs:range xsd:string ;
  skos:definition "Een toelichting op deze eigenschap en het belang hiervan voor zaak en van dit zaaktype."@nl ;
.
ztco:toelichtingZaaktype
  a owl:DatatypeProperty ;
  dcterms:modified "2019-03-20" ;
  rdfs:comment "De property toelichtingZaaktype wordt gebruikt om aan te geven welke toelichting is gekoppeld aan een zaaktype."@nl ;
  rdfs:domain ztco:Zaaktype ;
  rdfs:label "Toelichting zaaktype"@nl ;
  rdfs:range xsd:string ;
  skos:definition "Een eventuele toelichting op dit zaaktype. Dit attribuut heeft vooral een documentatiefunctie en is bedoeld om een toelichting te geven op dit zaaktype. Hier kan bijvoorbeeld een beschrijving van het procesverloop op hoofdlijnen worden gegeven. "@nl ;
.
ztco:typeOnderzoek
  a ztco:Eigenschaptype ;
  dcterms:modified "2019-03-27" ;
  rdfs:comment "De Eigenschaptype instantie typeOnderzoek wordt gebruikt om aan te geven welke type onderzoek is gekoppeld aan een zaak."@nl ;
  rdfs:label "Type onderzoek"@nl ;
  ztco:toelichtingEigenschaptype "De verschillende Archeologische Projecten binnen RCE"@nl ;
  ztco:waardenverzamelingEigenschaptype "ABE - Archeologisch: begeleiding;ABO - Archeologisch: booronderzoek;ABU - Archeologisch: bureauonderzoek;ADU - Archeologisch: duikactiviteiten;AGO - Archeologisch: geofysisch onderzoek;AIN - Archeologisch: inspectie;AKA - Archeologisch: (veld)kartering;AOP - Archeologisch: opgraving;AOW - Archeologisch: onderwaterarcheologie;APP - Archeologisch: proefputten/proefsleuven;AVE - Archeologisch: verwachtingskaart;AXX - Archeologisch: onbepaald;IAR - Indirect: archief;ICO - Indirect: collectie;ILI - Indirect: literatuur;IXX - Indirect: onbepaald;LUC - Luchtfoto/remote sensing;NBA - Niet-archeologisch: baggerwerk;NBO - Niet-archeologisch: boring;NDE - Niet-archeologisch: metaaldetector;NDU - Niet archeologisch: duikactiviteiten;NGR - Niet-archeologisch: graafwerk;NKA - Niet-archeologisch: kartering;NWA - Niet archeologisch: waterwerk en exploitatie;NXX - Niet-archeologisch: onbepaald;XXX - Onbekend" ;
.
ztco:url
  a owl:DatatypeProperty ;
  rdfs:comment "De property url wordt gebruikt om aan te geven welke url is gekoppeld aan een zaaktype."@nl ;
  rdfs:domain ztco:Zaaktype ;
  rdfs:label "URL"@nl ;
  rdfs:range xsd:string ;
  skos:definition "De URL naar het formulier."@nl ;
.
ztco:verantwoordelijke
  a owl:DatatypeProperty ;
  dcterms:modified "2019-03-25" ;
  rdfs:comment "De property verantwoordelijke wordt gebruikt om aan te geven welke verantwoordelijke organisatorische eenheid of medewerker is gekoppeld aan een zaaktype."@nl ;
  rdfs:domain ztco:Zaaktype ;
  rdfs:label "Verantwoordelijke"@nl ;
  rdfs:range xsd:string ;
  skos:definition "De verantwoordelijke organisatorische eenheid of medewerker voor zaken van het zaaktype."@nl ;
.
ztco:verplichtBijStatustype
  a owl:ObjectProperty ;
  dcterms:modified "2019-02-20" ;
  rdfs:comment "De property verplichtBijStatustype legt de relatie tussen documenttype en statustype vast."@nl ;
  rdfs:domain ztco:Documenttype ;
  rdfs:label "Verplicht bij statustype"@nl ;
  rdfs:range ztco:Statustype ;
  owl:inverseOf ztco:hoortBijDocumenttype ;
  skos:definition "De statustype waarvoor geldt dat er een document van dit documenttype verplicht aanwezig moet zijn in het zaakdossier van een zaak voordat de status van dit statustype kan worden gezet."@nl ;
.
ztco:vertrouwelijkAanduidingDocumenttype
  a owl:DatatypeProperty ;
  rdfs:comment "De property vertrouwelijkAanduiding wordt gebruikt om aan te geven welke vertrouwelijk aanduiding is gekoppeld aan een documenttype."@nl ;
  rdfs:domain ztco:Documenttype ;
  rdfs:label "Vertrouwelijk aanduiding documenttype"@nl ;
  rdfs:range xsd:string ;
  skos:definition "Aanduiding van de mate waarin documenten van dit documenttype voor de openbaarheid bestemd zijn. Middels deze attribuutsoort kan worden vastgelegd in welke mate documenten van dit documenttype bestemd zijn voor de openbaarheid. Zo kan een zaak waarvoor in het zaaktype is vastgelegd dat de Vertrouwelijkaanduiding 'Openbaar' is, toch documenten bevatten die op basis van hun documenttype niet - samen met de openbare zaakinformatie - 'Openbaar' worden gemaakt. "@nl ;
.
ztco:vertrouwelijkAanduidingZaaktype
  a owl:DatatypeProperty ;
  rdfs:comment "De property vertrouwelijkAanduidingZaaktype wordt gebruikt om aan te geven welke vertrouwelijk aanduiding is gekoppeld aan een zaaktype."@nl ;
  rdfs:domain ztco:Zaaktype ;
  rdfs:label "Vertrouwelijk aanduiding zaaktype"@nl ;
  rdfs:range xsd:string ;
  skos:definition "Aanduiding van de mate waarin zaakdossiers van zaken van dit zaaktype voor de openbaarheid bestemd zijn."@nl ;
.
ztco:waardenverzamelingEigenschaptype
  a owl:DatatypeProperty ;
  rdfs:comment "De property waardenverzamelingEigenschaptype wordt gebruikt om aan te geven welke waardenverzameling is gekoppeld aan een eigenschaptype."@nl ;
  rdfs:domain ztco:Eigenschaptype ;
  rdfs:label "Waardenverzameling eigenschaptype"@nl ;
  rdfs:range xsd:string ;
  skos:definition "De - verzameling van - waarden die gegevens van deze eigenschap kunnen hebben."@nl ;
.
ztco:wijzigingstype
  a ztco:Eigenschaptype ;
  dcterms:created "2019-03-27" ;
  dcterms:modified "" ;
  rdfs:comment "De Eigenschaptype instantie wijzigingstype wordt gebruikt om aan te geven welk wijzigingstype is gekoppeld aan een zaak."@nl ;
  rdfs:label "Wijzigingstype"@nl ;
  ztco:waardenverzamelingEigenschaptype "Gemeentelijke herindeling;Met Kadaster en/of afhandelingsbericht; Zonder Kadaster en afhandelingsbericht" ;
.
ztco:wordtVastgelegdInDocumenttype
  a owl:ObjectProperty ;
  rdfs:comment "De property wordtVastgelegdInDocumenttype legt de relatie tussen besluittype en documenttype vast."@nl ;
  rdfs:domain ztco:Besluittype ;
  rdfs:label "Wordt vastgelegd in documenttype"@nl ;
  rdfs:range ztco:Documenttype ;
  owl:inverseOf ztco:legtVastBesluit ;
  skos:definition "Het documenttype waarin besluiten van dit besluittype worden vastgelegd"@nl ;
.
ztco:zaaktypeOmschrijving
  a owl:DatatypeProperty ;
  dcterms:modified "2019-03-20" ;
  rdfs:comment "De property zaaktypeOmschrijving wordt gebruikt om aan te geven welke omschrijving is gekoppeld aan een zaaktype."@nl ;
  rdfs:domain ztco:Zaaktype ;
  rdfs:label "zaaktypeomschrijving"@nl ;
  rdfs:range xsd:string ;
  skos:definition "Korte omschrijving van de aard van zaaken van het zaaktype."@nl ;
.
ztco:zetAlsBetrokkeneStatustype
  a owl:ObjectProperty ;
  dcterms:modified "2019-02-20" ;
  rdfs:comment "De property zetAlsBetrokkeneStatustype legt de relatie tussen roltype en statustype vast."@nl ;
  rdfs:domain ztco:Roltype ;
  rdfs:label "Zet als betrokkene statustype"@nl ;
  rdfs:range ztco:Statustype ;
  owl:inverseOf ztco:isGezetDoorRoltype ;
  skos:definition "De statustypen die een betrokkene in een rol van dit roltype mag zetten"@nl ;
.
[
  a rdfs:Datatype ;
  owl:oneOf (
      "ABE - Archeologisch: begeleiding"
      "ABO - Archeologisch: booronderzoek"
      "ABU - Archeologisch: bureauonderzoek"
      "ADU - Archeologisch: duikactiviteiten"
      "AGO - Archeologisch: geofysisch onderzoek"
      "AIN - Archeologisch: inspectie"
      "AKA - Archeologisch: (veld)kartering"
      "AOP - Archeologisch: opgraving"
      "AOW - Archeologisch: onderwaterarcheologie"
      "APP - Archeologisch: proefputten/proefsleuven"
      "AVE - Archeologisch: verwachtingskaart"
      "AXX - Archeologisch: onbepaald"
      "IAR - Indirect: archief"
      "ICO - Indirect: collectie"
      "ILI - Indirect: literatuur"
      "IXX - Indirect: onbepaald"
      "LUC - Luchtfoto/remote sensing"
      "NBA - Niet-archeologisch: baggerwerk"
      "NBO - Niet-archeologisch: boring"
      "NDE - Niet-archeologisch: metaaldetector"
      "NDU - Niet archeologisch: duikactiviteiten"
      "NGR - Niet-archeologisch: graafwerk"
      "NKA - Niet-archeologisch: kartering"
      "NWA - Niet archeologisch: waterwerk en exploitatie"
      "NXX - Niet-archeologisch: onbepaald"
      "XXX - Onbekend"
    ) ;
].
[
  a rdfs:Datatype ;
  owl:oneOf (
      "Gemeente"
      "Waterschap"
      "Provincie"
      "Rijk"
      "Geen"
    ) ;
].
[
  a rdfs:Datatype ;
  owl:oneOf (
      "Kort"
      "Lang"
      "Administratief"
    ) ;
].
[
  a rdfs:Datatype ;
  owl:oneOf (
      "Monumentenwet 1988"
      "Erfgoedwet 2016"
    ) ;
].
[
  a rdfs:Datatype ;
  owl:oneOf (
      "Wederopbouw 1940-1958"
      "Nieuwe Hollandse Waterlinie"
      "MSP"
      "Archeologie 2008"
      "Archeologie 2013"
      "Wederopbouw 1959-1965"
      "WKPB"
      "Vestingwerken"
      "Verbetervoorstellen algemeen"
      "Verbetervoorstellen Molens"
      "Verbetervoorstellen Kerken"
      "Verbetervoorstellen Utrecht bruggen"
      "Verbetervoorstellen subsidies"
    ) ;
].
